Hashmap/DHashMap/Basic.lean
@@ -28,38 +28,38 @@ instance : EmptyCollection (Raw α β) where
     (Raw₀.insert ⟨m, h⟩ a b).1
   else m -- will never happen for well-formed inputs
 
-@[inline] def insertB [BEq α] [Hashable α] (m : Raw α β) (a : α) (b : β a) : Raw α β × Bool :=
+@[inline] def containsThenInsert [BEq α] [Hashable α] (m : Raw α β) (a : α) (b : β a) : Raw α β × Bool :=
   if h : 0 < m.buckets.size then
-    let ⟨⟨r, _⟩, replaced⟩ := Raw₀.insertB ⟨m, h⟩ a b
+    let ⟨⟨r, _⟩, replaced⟩ := Raw₀.containsThenInsert ⟨m, h⟩ a b
     ⟨r, replaced⟩
   else (m, false) -- will never happen for well-formed inputs
 
-@[inline] def computeIfAbsentM [BEq α] [Hashable α] [LawfulBEq α] {β : α → Type u} {m : Type u → Type v} [Monad m]
+@[inline] def insertIfNewThenGetM [BEq α] [Hashable α] [LawfulBEq α] {β : α → Type u} {m : Type u → Type v} [Monad m]
     (q : Raw α β) (a : α) (f : Unit → m (β a)) : m (Raw α β × β a) :=
   if h : 0 < q.buckets.size then do
-    let ⟨⟨r, _⟩, s⟩ ← Raw₀.computeIfAbsentM ⟨q, h⟩ a f
+    let ⟨⟨r, _⟩, s⟩ ← Raw₀.insertIfNewThenGetM ⟨q, h⟩ a f
     return (r, s)
   else return (q, ← f ()) -- will never happen for well-formed inputs
 
-@[inline] def computeIfAbsent [BEq α] [Hashable α] [LawfulBEq α] (m : Raw α β) (a : α) (f : Unit → β a) : Raw α β × β a :=
+@[inline] def insertIfNewThenGet [BEq α] [Hashable α] [LawfulBEq α] (m : Raw α β) (a : α) (f : Unit → β a) : Raw α β × β a :=
   if h : 0 < m.buckets.size then
-    let ⟨⟨r, _⟩, s⟩ := Raw₀.computeIfAbsent ⟨m, h⟩ a f
+    let ⟨⟨r, _⟩, s⟩ := Raw₀.insertIfNewThenGet ⟨m, h⟩ a f
     (r, s)
   else (m, f ()) -- will never happen for well-formed inputs
 
-@[inline] def findEntry? [BEq α] [Hashable α] (m : Raw α β) (a : α) : Option (Σ a, β a) :=
+@[inline] def getEntry? [BEq α] [Hashable α] (m : Raw α β) (a : α) : Option (Σ a, β a) :=
   if h : 0 < m.buckets.size then
-    Raw₀.findEntry? ⟨m, h⟩ a
+    Raw₀.getEntry? ⟨m, h⟩ a
   else none -- will never happen for well-formed inputs
 
-@[inline] def find? [BEq α] [LawfulBEq α] [Hashable α] (m : Raw α β) (a : α) : Option (β a) :=
+@[inline] def get? [BEq α] [LawfulBEq α] [Hashable α] (m : Raw α β) (a : α) : Option (β a) :=
   if h : 0 < m.buckets.size then
-    Raw₀.find? ⟨m, h⟩ a
+    Raw₀.get? ⟨m, h⟩ a
   else none -- will never happen for well-formed inputs
 
-@[inline] def findWithCast? [BEq α] [Hashable α] (m : Raw α β) (a : α) (cast : ∀ {b}, b == a → β b → β a) : Option (β a) :=
+@[inline] def getWithCast? [BEq α] [Hashable α] (m : Raw α β) (a : α) (cast : ∀ {b}, b == a → β b → β a) : Option (β a) :=
   if h : 0 < m.buckets.size then
-    Raw₀.findWithCast? ⟨m, h⟩ a cast
+    Raw₀.getWithCast? ⟨m, h⟩ a cast
   else none -- will never happen for well-formed inputs
 
 @[inline] def contains [BEq α] [Hashable α] (m : Raw α β) (a : α) : Bool :=
@@ -67,9 +67,9 @@ instance : EmptyCollection (Raw α β) where
     Raw₀.contains ⟨m, h⟩ a
   else false -- will never happen for well-formed inputs
 
-@[inline] def erase [BEq α] [Hashable α] (m : Raw α β) (a : α) : Raw α β :=
+@[inline] def remove [BEq α] [Hashable α] (m : Raw α β) (a : α) : Raw α β :=
   if h : 0 < m.buckets.size then
-    Raw₀.erase ⟨m, h⟩ a
+    Raw₀.remove ⟨m, h⟩ a
   else m -- will never happen for well-formed inputs
 
 @[inline] def filterMap {γ : α → Type w} (f : (a : α) → β a → Option (γ a)) (m : Raw α β) : Raw α γ :=
@@ -86,9 +86,9 @@ section
 
 variable {β : Type v}
 
-@[inline] def findConst? [BEq α] [Hashable α] (m : Raw α (fun _ => β)) (a : α) : Option β :=
+@[inline] def Const.get? [BEq α] [Hashable α] (m : Raw α (fun _ => β)) (a : α) : Option β :=
   if h : 0 < m.buckets.size then
-    Raw₀.findConst? ⟨m, h⟩ a
+    Raw₀.Const.get? ⟨m, h⟩ a
   else none -- will never happen for well-formed inputs
 
 end
@@ -102,7 +102,7 @@ def foldl (f : δ → (a : α) → β a → δ) (init : δ) (b : Raw α β) : δ
   Id.run (b.foldlM f init)
 
 def beq [BEq α] [Hashable α] [LawfulBEq α] [∀ k, BEq (β k)] (m₁ m₂ : Raw α β) : Bool :=
-  m₁.size = m₂.size && (m₁.foldl fun acc k v => acc && match m₂.find? k with
+  m₁.size = m₂.size && (m₁.foldl fun acc k v => acc && match m₂.get? k with
   | none => false
   | some v' => v == v') true
 
@@ -148,17 +148,17 @@ inductive WF [BEq α] [Hashable α] : Raw α β → Prop where
   | wf {m} : 0 < m.buckets.size → (∀ [EquivBEq α] [LawfulHashable α], m.WFImp) → WF m
   | empty₀ {c} : WF (Raw₀.empty c).1
   | insert₀ {m h a b} : WF m → WF (Raw₀.insert ⟨m, h⟩ a b).1
-  | insertB₀ {m h a b} : WF m → WF (Raw₀.insertB ⟨m, h⟩ a b).1.1
-  | erase₀ {m h a} : WF m → WF (Raw₀.erase ⟨m, h⟩ a).1
-  | computeIfAbsent₀ [LawfulBEq α] {m h a f} : WF m → WF (Raw₀.computeIfAbsent ⟨m, h⟩ a f).1
+  | containsThenInsert₀ {m h a b} : WF m → WF (Raw₀.containsThenInsert ⟨m, h⟩ a b).1.1
+  | remove₀ {m h a} : WF m → WF (Raw₀.remove ⟨m, h⟩ a).1
+  | insertIfNewThenGet₀ [LawfulBEq α] {m h a f} : WF m → WF (Raw₀.insertIfNewThenGet ⟨m, h⟩ a f).1
 
 theorem WF.size_buckets_pos [BEq α] [Hashable α] (m : Raw α β) : WF m → 0 < m.buckets.size
   | wf h₁ _ => h₁
   | empty₀ => (Raw₀.empty _).2
   | insert₀ _ => (Raw₀.insert ⟨_, _⟩ _ _).2
-  | insertB₀ _ => (Raw₀.insertB ⟨_, _⟩ _ _).1.2
-  | erase₀ _ => (Raw₀.erase ⟨_, _⟩ _).2
-  | computeIfAbsent₀ _ => (Raw₀.computeIfAbsent ⟨_, _⟩ _ _).1.2
+  | containsThenInsert₀ _ => (Raw₀.containsThenInsert ⟨_, _⟩ _ _).1.2
+  | remove₀ _ => (Raw₀.remove ⟨_, _⟩ _).2
+  | insertIfNewThenGet₀ _ => (Raw₀.insertIfNewThenGet ⟨_, _⟩ _ _).1.2
 
 @[simp]
 theorem WF.empty [BEq α] [Hashable α] {c : Nat} : (Raw.empty c : Raw α β).WF :=
@@ -168,14 +168,14 @@ theorem WF.empty [BEq α] [Hashable α] {c : Nat} : (Raw.empty c : Raw α β).WF
 theorem WF.emptyc [BEq α] [Hashable α] : (∅ : Raw α β).WF :=
   .empty
 
-theorem WF.insertB [BEq α] [Hashable α] {m : Raw α β} {a : α} {b : β a} (h : m.WF) : (m.insertB a b).1.WF := by
-  simpa [Raw.insertB, h.size_buckets_pos] using .insertB₀ h
+theorem WF.containsThenInsert [BEq α] [Hashable α] {m : Raw α β} {a : α} {b : β a} (h : m.WF) : (m.containsThenInsert a b).1.WF := by
+  simpa [Raw.containsThenInsert, h.size_buckets_pos] using .containsThenInsert₀ h
 
 theorem WF.insert [BEq α] [Hashable α] {m : Raw α β} {a : α} {b : β a} (h : m.WF) : (m.insert a b).WF := by
   simpa [Raw.insert, h.size_buckets_pos] using .insert₀ h
 
-theorem WF.erase [BEq α] [Hashable α] {m : Raw α β} {a : α} (h : m.WF) : (m.erase a).WF := by
-  simpa [Raw.erase, h.size_buckets_pos] using .erase₀ h
+theorem WF.remove [BEq α] [Hashable α] {m : Raw α β} {a : α} (h : m.WF) : (m.remove a).WF := by
+  simpa [Raw.remove, h.size_buckets_pos] using .remove₀ h
 
 end WF
 
@@ -198,9 +198,9 @@ instance [BEq α] [Hashable α] : EmptyCollection (DHashMap α β) where
 Inserts the mapping into the map, replacing an existing mapping if there is one.
 Returns `true` if there was a previous mapping that was replaced.
 -/
-@[inline] def insertB [BEq α] [Hashable α] (m : DHashMap α β) (a : α) (b : β a) : DHashMap α β × Bool :=
-  let m' := Raw₀.insertB ⟨m.1, m.2.size_buckets_pos⟩ a b
-  ⟨⟨m'.1.1, .insertB₀ m.2⟩, m'.2⟩
+@[inline] def containsThenInsert [BEq α] [Hashable α] (m : DHashMap α β) (a : α) (b : β a) : DHashMap α β × Bool :=
+  let m' := Raw₀.containsThenInsert ⟨m.1, m.2.size_buckets_pos⟩ a b
+  ⟨⟨m'.1.1, .containsThenInsert₀ m.2⟩, m'.2⟩
 
 /--
 Inserts the mapping into the map, replacing an existing mapping if there is one.
@@ -212,31 +212,31 @@ Inserts the mapping into the map, replacing an existing mapping if there is one.
 If the map contains a mapping for the given key, return the value. Otherwise, compute the value using the
 given function, insert it into the map, and return the value.
 -/
-@[inline] def computeIfAbsent [BEq α] [LawfulBEq α] [Hashable α] (m : DHashMap α β) (a : α) (f : Unit → β a) : DHashMap α β × β a :=
-  let m' := Raw₀.computeIfAbsent ⟨m.1, m.2.size_buckets_pos⟩ a f
-  ⟨⟨m'.1.1, .computeIfAbsent₀ m.2⟩, m'.2⟩
+@[inline] def insertIfNewThenGet [BEq α] [LawfulBEq α] [Hashable α] (m : DHashMap α β) (a : α) (f : Unit → β a) : DHashMap α β × β a :=
+  let m' := Raw₀.insertIfNewThenGet ⟨m.1, m.2.size_buckets_pos⟩ a f
+  ⟨⟨m'.1.1, .insertIfNewThenGet₀ m.2⟩, m'.2⟩
 
 /--
 Retrieves the mapping associated with the given key, if it exists.
 -/
-@[inline] def findEntry? [BEq α] [Hashable α] (m : DHashMap α β) (a : α) : Option (Σ a, β a) :=
-  Raw₀.findEntry? ⟨m.1, m.2.size_buckets_pos⟩ a
+@[inline] def getEntry? [BEq α] [Hashable α] (m : DHashMap α β) (a : α) : Option (Σ a, β a) :=
+  Raw₀.getEntry? ⟨m.1, m.2.size_buckets_pos⟩ a
 
 /--
 Retrieves the value associated with the given key, if it exists. This function requires a `LawfulBEq` instance
-to be able to cast the value to the correct type. If no such instance is available, you can use `findEntry?`,
-`findWithCast?`,
+to be able to cast the value to the correct type. If no such instance is available, you can use `getEntry?`,
+`getWithCast?`,
 or switch to a non-dependent `HashMap`.
 -/
-@[inline] def find? [BEq α] [LawfulBEq α] [Hashable α] (m : DHashMap α β) (a : α) : Option (β a) :=
-  Raw₀.find? ⟨m.1, m.2.size_buckets_pos⟩ a
+@[inline] def get? [BEq α] [LawfulBEq α] [Hashable α] (m : DHashMap α β) (a : α) : Option (β a) :=
+  Raw₀.get? ⟨m.1, m.2.size_buckets_pos⟩ a
 
 /--
 Retrieves the value associated with the given key, if it exists, and casts the value to the correct dependent type using
 the provided cast function.
 -/
-@[inline] def findWithCast? [BEq α] [Hashable α] (m : DHashMap α β) (a : α) (cast : ∀ {b}, b == a → β b → β a) : Option (β a) :=
-  Raw₀.findWithCast? ⟨m.1, m.2.size_buckets_pos⟩ a cast
+@[inline] def getWithCast? [BEq α] [Hashable α] (m : DHashMap α β) (a : α) (cast : ∀ {b}, b == a → β b → β a) : Option (β a) :=
+  Raw₀.getWithCast? ⟨m.1, m.2.size_buckets_pos⟩ a cast
 
 /-- Returns true if the hash map contains a mapping with a key equal to the given key. -/
 @[inline] def contains [BEq α] [Hashable α] (m : DHashMap α β) (a : α) : Bool :=
@@ -248,8 +248,8 @@ the provided cast function.
 /--
 Removes the mapping with the given key if it exists.
 -/
-@[inline] def erase [BEq α] [Hashable α] (m : DHashMap α β) (a : α) : DHashMap α β :=
-  ⟨Raw₀.erase ⟨m.1, m.2.size_buckets_pos⟩ a, .erase₀ m.2⟩
+@[inline] def remove [BEq α] [Hashable α] (m : DHashMap α β) (a : α) : DHashMap α β :=
+  ⟨Raw₀.remove ⟨m.1, m.2.size_buckets_pos⟩ a, .remove₀ m.2⟩
 
 section
 
@@ -257,8 +257,8 @@ variable {β : Type v}
 
 /--
 Retrieves the value associated with the given key, if it exists. -/
-@[inline] def findConst? [BEq α] [Hashable α] (m : DHashMap α (fun _ => β)) (a : α) : Option β :=
-  Raw₀.findConst? ⟨m.1, m.2.size_buckets_pos⟩ a
+@[inline] def Const.get? [BEq α] [Hashable α] (m : DHashMap α (fun _ => β)) (a : α) : Option β :=
+  Raw₀.Const.get? ⟨m.1, m.2.size_buckets_pos⟩ a
 
 end
 
