Hashmap/List/Associative.lean
@@ -38,132 +38,132 @@ theorem assoc_induction {motive : List (Σ a, β a) → Prop} (nil : motive [])
   | ⟨_, _⟩ :: _ => cons _ _ _ (assoc_induction nil cons _)
 
 /-- Search for an entry in a list of dependent pairs by key. -/
-def findEntry? [BEq α] (a : α) : List (Σ a, β a) → Option (Σ a, β a)
+def getEntry? [BEq α] (a : α) : List (Σ a, β a) → Option (Σ a, β a)
   | [] => none
-  | ⟨k, v⟩ :: l => bif k == a then some ⟨k, v⟩ else findEntry? a l
+  | ⟨k, v⟩ :: l => bif k == a then some ⟨k, v⟩ else getEntry? a l
 
-@[simp] theorem findEntry?_nil [BEq α] {a : α} : ([] : List (Σ a, β a)).findEntry? a = none := rfl
-theorem findEntry?_cons [BEq α] {l : List (Σ a, β a)} {k a : α} {v : β k} :
-    (⟨k, v⟩ :: l).findEntry? a = bif k == a then some ⟨k, v⟩ else l.findEntry? a := rfl
+@[simp] theorem getEntry?_nil [BEq α] {a : α} : ([] : List (Σ a, β a)).getEntry? a = none := rfl
+theorem getEntry?_cons [BEq α] {l : List (Σ a, β a)} {k a : α} {v : β k} :
+    (⟨k, v⟩ :: l).getEntry? a = bif k == a then some ⟨k, v⟩ else l.getEntry? a := rfl
 
-theorem findEntry?_cons_of_true [BEq α] {l : List (Σ a, β a)} {k a : α} {v : β k} (h : k == a) :
-    (⟨k, v⟩ :: l).findEntry? a = some ⟨k, v⟩ := by
-  simp [findEntry?, h]
+theorem getEntry?_cons_of_true [BEq α] {l : List (Σ a, β a)} {k a : α} {v : β k} (h : k == a) :
+    (⟨k, v⟩ :: l).getEntry? a = some ⟨k, v⟩ := by
+  simp [getEntry?, h]
 
-theorem findEntry?_cons_of_false [BEq α] {l : List (Σ a, β a)} {k a : α} {v : β k} (h : (k == a) = false) :
-    (⟨k, v⟩ :: l).findEntry? a = l.findEntry? a := by
-  simp [findEntry?, h]
+theorem getEntry?_cons_of_false [BEq α] {l : List (Σ a, β a)} {k a : α} {v : β k} (h : (k == a) = false) :
+    (⟨k, v⟩ :: l).getEntry? a = l.getEntry? a := by
+  simp [getEntry?, h]
 
 @[simp]
-theorem findEntry?_cons_self [BEq α] [ReflBEq α] {l : List (Σ a, β a)} {k : α} {v : β k} :
-    (⟨k, v⟩ :: l).findEntry? k = some ⟨k, v⟩ :=
-  findEntry?_cons_of_true BEq.refl
+theorem getEntry?_cons_self [BEq α] [ReflBEq α] {l : List (Σ a, β a)} {k : α} {v : β k} :
+    (⟨k, v⟩ :: l).getEntry? k = some ⟨k, v⟩ :=
+  getEntry?_cons_of_true BEq.refl
 
-theorem findEntry?_eq_some [BEq α] {l : List (Σ a, β a)} {a : α} {p : Σ a, β a}
-    (h : l.findEntry? a = some p) : p.1 == a := by
+theorem getEntry?_eq_some [BEq α] {l : List (Σ a, β a)} {a : α} {p : Σ a, β a}
+    (h : l.getEntry? a = some p) : p.1 == a := by
   induction l using assoc_induction
   · simp at h
   · next k' v' t ih =>
     cases h' : k' == a
-    · rw [findEntry?_cons_of_false h'] at h
+    · rw [getEntry?_cons_of_false h'] at h
       exact ih h
-    · rw [findEntry?_cons_of_true h', Option.some.injEq] at h
+    · rw [getEntry?_cons_of_true h', Option.some.injEq] at h
       obtain rfl := congrArg Sigma.fst h
       exact h'
 
-theorem findEntry?_eq_of_beq [BEq α] [PartialEquivBEq α] {l : List (Σ a, β a)} {a a' : α} (h : a == a') :
-    l.findEntry? a = l.findEntry? a' := by
+theorem getEntry?_eq_of_beq [BEq α] [PartialEquivBEq α] {l : List (Σ a, β a)} {a a' : α} (h : a == a') :
+    l.getEntry? a = l.getEntry? a' := by
   induction l using assoc_induction
   · simp
   · next k v l ih =>
     cases h' : k == a
     · have h₂ : (k == a') = false := BEq.neq_of_neq_of_beq h' h
-      rw [findEntry?_cons_of_false h', findEntry?_cons_of_false h₂, ih]
-    · rw [findEntry?_cons_of_true h', findEntry?_cons_of_true (BEq.trans h' h)]
+      rw [getEntry?_cons_of_false h', getEntry?_cons_of_false h₂, ih]
+    · rw [getEntry?_cons_of_true h', getEntry?_cons_of_true (BEq.trans h' h)]
 
 section
 
 variable {β : Type v}
 
-def findValue? [BEq α] (a : α) : List ((_ : α) × β) → Option β
+def getValue? [BEq α] (a : α) : List ((_ : α) × β) → Option β
   | [] => none
-  | ⟨k, v⟩ :: l => bif k == a then some v else l.findValue? a
+  | ⟨k, v⟩ :: l => bif k == a then some v else l.getValue? a
 
-@[simp] theorem findValue?_nil [BEq α] {a : α} : ([] : List ((_ : α) × β)).findValue? a = none := rfl
-theorem findValue?_cons [BEq α] {l : List ((_ : α) × β)} {k a : α} {v : β} :
-    (⟨k, v⟩ :: l).findValue? a = bif k == a then some v else l.findValue? a := rfl
+@[simp] theorem getValue?_nil [BEq α] {a : α} : ([] : List ((_ : α) × β)).getValue? a = none := rfl
+theorem getValue?_cons [BEq α] {l : List ((_ : α) × β)} {k a : α} {v : β} :
+    (⟨k, v⟩ :: l).getValue? a = bif k == a then some v else l.getValue? a := rfl
 
-theorem findValue?_cons_of_true [BEq α] {l : List ((_ : α) × β)} {k a : α} {v : β} (h : k == a) :
-    (⟨k, v⟩ :: l).findValue? a = some v := by
-  simp [findValue?, h]
+theorem getValue?_cons_of_true [BEq α] {l : List ((_ : α) × β)} {k a : α} {v : β} (h : k == a) :
+    (⟨k, v⟩ :: l).getValue? a = some v := by
+  simp [getValue?, h]
 
-theorem findValue?_cons_of_false [BEq α] {l : List ((_ : α) × β)} {k a : α} {v : β} (h : (k == a) = false) :
-    (⟨k, v⟩ :: l).findValue? a = l.findValue? a := by
-  simp [findValue?, h]
+theorem getValue?_cons_of_false [BEq α] {l : List ((_ : α) × β)} {k a : α} {v : β} (h : (k == a) = false) :
+    (⟨k, v⟩ :: l).getValue? a = l.getValue? a := by
+  simp [getValue?, h]
 
 @[simp]
-theorem findValue?_cons_self [BEq α] [ReflBEq α] {l : List ((_ : α) × β)} {k : α} {v : β} :
-    (⟨k, v⟩ :: l).findValue? k = some v :=
-  findValue?_cons_of_true BEq.refl
+theorem getValue?_cons_self [BEq α] [ReflBEq α] {l : List ((_ : α) × β)} {k : α} {v : β} :
+    (⟨k, v⟩ :: l).getValue? k = some v :=
+  getValue?_cons_of_true BEq.refl
 
-theorem findValue?_eq_findEntry? [BEq α] {l : List ((_ : α) × β)} {a : α} :
-    l.findValue? a = (l.findEntry? a).map (·.2) := by
+theorem getValue?_eq_getEntry? [BEq α] {l : List ((_ : α) × β)} {a : α} :
+    l.getValue? a = (l.getEntry? a).map (·.2) := by
   induction l using assoc_induction
   · simp
   · next k v l ih =>
     cases h : k == a
-    · rw [findEntry?_cons_of_false h, findValue?_cons_of_false h, ih]
-    · rw [findEntry?_cons_of_true h, findValue?_cons_of_true h, Option.map_some']
+    · rw [getEntry?_cons_of_false h, getValue?_cons_of_false h, ih]
+    · rw [getEntry?_cons_of_true h, getValue?_cons_of_true h, Option.map_some']
 
-theorem findValue?_eq_of_beq [BEq α] [PartialEquivBEq α] {l : List ((_ : α) × β)} {a a' : α} (h : a == a') :
-    l.findValue? a = l.findValue? a' := by
-  simp [findValue?_eq_findEntry?, findEntry?_eq_of_beq h]
+theorem getValue?_eq_of_beq [BEq α] [PartialEquivBEq α] {l : List ((_ : α) × β)} {a a' : α} (h : a == a') :
+    l.getValue? a = l.getValue? a' := by
+  simp [getValue?_eq_getEntry?, getEntry?_eq_of_beq h]
 
 end
 
-def findValueCast? [BEq α] [LawfulBEq α] (a : α) : List (Σ a, β a) → Option (β a)
+def getValueCast? [BEq α] [LawfulBEq α] (a : α) : List (Σ a, β a) → Option (β a)
   | [] => none
-  | ⟨k, v⟩ :: l => if h : k == a then some (cast (congrArg β (eq_of_beq h)) v) else l.findValueCast? a
+  | ⟨k, v⟩ :: l => if h : k == a then some (cast (congrArg β (eq_of_beq h)) v) else l.getValueCast? a
 
-@[simp] theorem findValueCast?_nil [BEq α] [LawfulBEq α] {a : α} :
-    ([] : List (Σ a, β a)).findValueCast? a = none := rfl
-theorem findValueCast?_cons [BEq α] [LawfulBEq α] {l : List (Σ a, β a)} {k a : α} {v : β k} :
-    (⟨k, v⟩ :: l).findValueCast? a = if h : k == a then some (cast (congrArg β (eq_of_beq h)) v) else l.findValueCast? a := rfl
+@[simp] theorem getValueCast?_nil [BEq α] [LawfulBEq α] {a : α} :
+    ([] : List (Σ a, β a)).getValueCast? a = none := rfl
+theorem getValueCast?_cons [BEq α] [LawfulBEq α] {l : List (Σ a, β a)} {k a : α} {v : β k} :
+    (⟨k, v⟩ :: l).getValueCast? a = if h : k == a then some (cast (congrArg β (eq_of_beq h)) v) else l.getValueCast? a := rfl
 
-theorem findValueCast?_cons_of_true [BEq α] [LawfulBEq α] {l : List (Σ a, β a)} {k a : α} {v : β k} (h : k == a) :
-    (⟨k, v⟩ :: l).findValueCast? a = some (cast (congrArg β (eq_of_beq h)) v) := by
-  simp [findValueCast?, h]
+theorem getValueCast?_cons_of_true [BEq α] [LawfulBEq α] {l : List (Σ a, β a)} {k a : α} {v : β k} (h : k == a) :
+    (⟨k, v⟩ :: l).getValueCast? a = some (cast (congrArg β (eq_of_beq h)) v) := by
+  simp [getValueCast?, h]
 
-theorem findValueCast?_cons_of_false [BEq α] [LawfulBEq α] {l : List (Σ a, β a)} {k a : α} {v : β k}
-    (h : (k == a) = false) : (⟨k, v⟩ :: l).findValueCast? a = l.findValueCast? a := by
-  simp [findValueCast?, h]
+theorem getValueCast?_cons_of_false [BEq α] [LawfulBEq α] {l : List (Σ a, β a)} {k a : α} {v : β k}
+    (h : (k == a) = false) : (⟨k, v⟩ :: l).getValueCast? a = l.getValueCast? a := by
+  simp [getValueCast?, h]
 
 @[simp]
-theorem findValueCast?_cons_self [BEq α] [LawfulBEq α] {l : List (Σ a, β a)} {k : α} {v : β k} :
-    (⟨k, v⟩ :: l).findValueCast? k = some v := by
-  rw [findValueCast?_cons_of_true BEq.refl, cast_eq]
+theorem getValueCast?_cons_self [BEq α] [LawfulBEq α] {l : List (Σ a, β a)} {k : α} {v : β k} :
+    (⟨k, v⟩ :: l).getValueCast? k = some v := by
+  rw [getValueCast?_cons_of_true BEq.refl, cast_eq]
 
-def findValueWithCast? [BEq α] (a : α) (cast : ∀ {b}, b == a → β b → β a) : List (Σ a, β a) → Option (β a)
+def getValueWithCast? [BEq α] (a : α) (cast : ∀ {b}, b == a → β b → β a) : List (Σ a, β a) → Option (β a)
   | [] => none
-  | ⟨k, v⟩ :: l => if h : k == a then some (cast h v) else l.findValueWithCast? a cast
+  | ⟨k, v⟩ :: l => if h : k == a then some (cast h v) else l.getValueWithCast? a cast
 
-@[simp] theorem findValueWithCast?_nil [BEq α] {a : α} {cast : ∀ {b}, b == a → β b → β a} :
-    ([] : List (Σ a, β a)).findValueWithCast? a cast = none := rfl
-theorem findValueWithCast?_cons [BEq α] {l : List (Σ a, β a)} {k a : α} {v : β k} {cast : ∀ {b}, b == a → β b → β a} :
-    (⟨k, v⟩ :: l).findValueWithCast? a cast = if h : k == a then some (cast h v) else l.findValueWithCast? a cast := rfl
+@[simp] theorem getValueWithCast?_nil [BEq α] {a : α} {cast : ∀ {b}, b == a → β b → β a} :
+    ([] : List (Σ a, β a)).getValueWithCast? a cast = none := rfl
+theorem getValueWithCast?_cons [BEq α] {l : List (Σ a, β a)} {k a : α} {v : β k} {cast : ∀ {b}, b == a → β b → β a} :
+    (⟨k, v⟩ :: l).getValueWithCast? a cast = if h : k == a then some (cast h v) else l.getValueWithCast? a cast := rfl
 
-theorem findValueWithCast?_cons_of_true [BEq α] {l : List (Σ a, β a)} {k a : α} {v : β k} {cast : ∀ {b}, b == a → β b → β a} (h : k == a) :
-    (⟨k, v⟩ :: l).findValueWithCast? a cast = some (cast h v) := by
-  simp [findValueWithCast?, h]
+theorem getValueWithCast?_cons_of_true [BEq α] {l : List (Σ a, β a)} {k a : α} {v : β k} {cast : ∀ {b}, b == a → β b → β a} (h : k == a) :
+    (⟨k, v⟩ :: l).getValueWithCast? a cast = some (cast h v) := by
+  simp [getValueWithCast?, h]
 
-theorem findValueWithCast?_cons_of_false [BEq α] {l : List (Σ a, β a)} {k a : α} {v : β k} {cast : ∀ {b}, b == a → β b → β a}
-    (h : (k == a) = false) : (⟨k, v⟩ :: l).findValueWithCast? a cast = l.findValueWithCast? a cast := by
-  simp [findValueWithCast?, h]
+theorem getValueWithCast?_cons_of_false [BEq α] {l : List (Σ a, β a)} {k a : α} {v : β k} {cast : ∀ {b}, b == a → β b → β a}
+    (h : (k == a) = false) : (⟨k, v⟩ :: l).getValueWithCast? a cast = l.getValueWithCast? a cast := by
+  simp [getValueWithCast?, h]
 
 @[simp]
-theorem findValueWithCast?_cons_self [BEq α] [ReflBEq α] {l : List (Σ a, β a)} {k : α} {v : β k} {cast : ∀ {b}, b == k → β b → β k} :
-    (⟨k, v⟩ :: l).findValueWithCast? k cast = some (cast BEq.refl v) := by
-  rw [findValueWithCast?_cons_of_true BEq.refl]
+theorem getValueWithCast?_cons_self [BEq α] [ReflBEq α] {l : List (Σ a, β a)} {k : α} {v : β k} {cast : ∀ {b}, b == k → β b → β k} :
+    (⟨k, v⟩ :: l).getValueWithCast? k cast = some (cast BEq.refl v) := by
+  rw [getValueWithCast?_cons_of_true BEq.refl]
 
 section
 
@@ -203,57 +203,57 @@ theorem _root_.Option.dmap_or {o o' : Option α} (f : (a : α) → ((o.or o') = 
 
 end
 
-theorem findValueCast?_eq_findEntry? [BEq α] [LawfulBEq α] {l : List (Σ a, β a)} {a : α} :
-    l.findValueCast? a = (l.findEntry? a).dmap (fun p h => cast (congrArg β (eq_of_beq (findEntry?_eq_some h))) p.2) := by
+theorem getValueCast?_eq_getEntry? [BEq α] [LawfulBEq α] {l : List (Σ a, β a)} {a : α} :
+    l.getValueCast? a = (l.getEntry? a).dmap (fun p h => cast (congrArg β (eq_of_beq (getEntry?_eq_some h))) p.2) := by
   induction l using assoc_induction
   · simp
   · next k v t ih =>
     cases h : k == a
-    · rw [findValueCast?_cons_of_false h, ih, Option.dmap_congr (findEntry?_cons_of_false h)]
-    · rw [findValueCast?_cons_of_true h, Option.dmap_congr (findEntry?_cons_of_true h), Option.dmap_some]
+    · rw [getValueCast?_cons_of_false h, ih, Option.dmap_congr (getEntry?_cons_of_false h)]
+    · rw [getValueCast?_cons_of_true h, Option.dmap_congr (getEntry?_cons_of_true h), Option.dmap_some]
 
-theorem isSome_findValueCast?_eq_isSome_findEntry? [BEq α] [LawfulBEq α] {l : List (Σ a, β a)} {a : α} :
-    (l.findValueCast? a).isSome = (l.findEntry? a).isSome := by
-  rw [findValueCast?_eq_findEntry?, Option.isSome_dmap]
+theorem isSome_getValueCast?_eq_isSome_getEntry? [BEq α] [LawfulBEq α] {l : List (Σ a, β a)} {a : α} :
+    (l.getValueCast? a).isSome = (l.getEntry? a).isSome := by
+  rw [getValueCast?_eq_getEntry?, Option.isSome_dmap]
 
-theorem findValueCast?_congr [BEq α] [LawfulBEq α] {l : List (Σ a, β a)} {a a' : α} (h : a == a') :
-    l.findValueCast? a = cast (congrArg _ (congrArg _ (eq_of_beq h).symm)) (l.findValueCast? a') := by
+theorem getValueCast?_congr [BEq α] [LawfulBEq α] {l : List (Σ a, β a)} {a a' : α} (h : a == a') :
+    l.getValueCast? a = cast (congrArg _ (congrArg _ (eq_of_beq h).symm)) (l.getValueCast? a') := by
   obtain rfl := eq_of_beq h
   rw [cast_eq]
 
-def findKey? [BEq α] (a : α) : List (Σ a, β a) → Option α
+def getKey? [BEq α] (a : α) : List (Σ a, β a) → Option α
   | nil => none
-  | ⟨k, _⟩ :: l => bif k == a then some k else l.findKey? a
+  | ⟨k, _⟩ :: l => bif k == a then some k else l.getKey? a
 
-@[simp] theorem findKey?_nil [BEq α] {a : α} : (nil : List (Σ a, β a)).findKey? a = none := rfl
-theorem findKey?_cons [BEq α] {l : List (Σ a, β a)} {k a : α} {v : β k} :
-    (⟨k, v⟩ :: l).findKey? a = bif k == a then some k else l.findKey? a := rfl
+@[simp] theorem getKey?_nil [BEq α] {a : α} : (nil : List (Σ a, β a)).getKey? a = none := rfl
+theorem getKey?_cons [BEq α] {l : List (Σ a, β a)} {k a : α} {v : β k} :
+    (⟨k, v⟩ :: l).getKey? a = bif k == a then some k else l.getKey? a := rfl
 
-theorem findKey?_cons_of_true [BEq α] {l : List (Σ a, β a)} {k a : α} {v : β k} (h : k == a) :
-    (⟨k, v⟩ :: l).findKey? a = some k := by
-  simp [findKey?, h]
+theorem getKey?_cons_of_true [BEq α] {l : List (Σ a, β a)} {k a : α} {v : β k} (h : k == a) :
+    (⟨k, v⟩ :: l).getKey? a = some k := by
+  simp [getKey?, h]
 
-theorem findKey?_cons_of_false [BEq α] {l : List (Σ a, β a)} {k a : α} {v : β k} (h : (k == a) = false) :
-    (⟨k, v⟩ :: l).findKey? a = l.findKey? a := by
-  simp [findKey?, h]
+theorem getKey?_cons_of_false [BEq α] {l : List (Σ a, β a)} {k a : α} {v : β k} (h : (k == a) = false) :
+    (⟨k, v⟩ :: l).getKey? a = l.getKey? a := by
+  simp [getKey?, h]
 
 @[simp]
-theorem findKey?_cons_self [BEq α] [ReflBEq α] {l : List (Σ a, β a)} {k : α} {v : β k} :
-    (⟨k, v⟩ :: l).findKey? k = k :=
-  findKey?_cons_of_true BEq.refl
+theorem getKey?_cons_self [BEq α] [ReflBEq α] {l : List (Σ a, β a)} {k : α} {v : β k} :
+    (⟨k, v⟩ :: l).getKey? k = k :=
+  getKey?_cons_of_true BEq.refl
 
-theorem findKey?_eq_findEntry? [BEq α] {l : List (Σ a, β a)} {a : α} :
-    l.findKey? a = (l.findEntry? a).map (·.1) := by
+theorem getKey?_eq_getEntry? [BEq α] {l : List (Σ a, β a)} {a : α} :
+    l.getKey? a = (l.getEntry? a).map (·.1) := by
   induction l using assoc_induction
   · simp
   · next k v l ih =>
     cases h : k == a
-    · rw [findEntry?_cons_of_false h, findKey?_cons_of_false h, ih]
-    · rw [findEntry?_cons_of_true h, findKey?_cons_of_true h, Option.map_some']
+    · rw [getEntry?_cons_of_false h, getKey?_cons_of_false h, ih]
+    · rw [getEntry?_cons_of_true h, getKey?_cons_of_true h, Option.map_some']
 
-theorem findKey?_eq_of_beq [BEq α] [PartialEquivBEq α] {l : List (Σ a, β a)} {a a' : α} (h : a == a') :
-    l.findKey? a = l.findKey? a' := by
-  simp [findKey?_eq_findEntry?, findEntry?_eq_of_beq h]
+theorem getKey?_eq_of_beq [BEq α] [PartialEquivBEq α] {l : List (Σ a, β a)} {a a' : α} (h : a == a') :
+    l.getKey? a = l.getKey? a' := by
+  simp [getKey?_eq_getEntry?, getEntry?_eq_of_beq h]
 
 def containsKey [BEq α] (a : α) : List (Σ a, β a) → Bool
   | nil => false
@@ -287,136 +287,136 @@ theorem containsKey_of_containsKey_cons [BEq α] {l : List (Σ a, β a)} {k a : 
   · exact False.elim (Bool.eq_false_iff.1 h₂ h)
   · exact h
 
-theorem containsKey_eq_isSome_findEntry? [BEq α] {l : List (Σ a, β a)} {a : α} :
-    l.containsKey a = (l.findEntry? a).isSome := by
+theorem containsKey_eq_isSome_getEntry? [BEq α] {l : List (Σ a, β a)} {a : α} :
+    l.containsKey a = (l.getEntry? a).isSome := by
   induction l using assoc_induction
   · simp
   · next k v l ih =>
     cases h : k == a
-    · simp [findEntry?_cons_of_false h, h, ih]
-    · simp [findEntry?_cons_of_true h, h]
+    · simp [getEntry?_cons_of_false h, h, ih]
+    · simp [getEntry?_cons_of_true h, h]
 
 theorem isEmpty_eq_false_of_containsKey [BEq α] {l : List (Σ a, β a)} {a : α} (h : l.containsKey a = true) :
     l.isEmpty = false := by
   cases l <;> simp_all
 
 @[simp]
-theorem findEntry?_eq_none [BEq α] {l : List (Σ a, β a)} {a : α} :
-    l.findEntry? a = none ↔ l.containsKey a = false := by
-  rw [← Option.not_isSome_iff_eq_none, Bool.not_eq_true, ← containsKey_eq_isSome_findEntry?]
+theorem getEntry?_eq_none [BEq α] {l : List (Σ a, β a)} {a : α} :
+    l.getEntry? a = none ↔ l.containsKey a = false := by
+  rw [← Option.not_isSome_iff_eq_none, Bool.not_eq_true, ← containsKey_eq_isSome_getEntry?]
 
 @[simp]
-theorem findKey?_eq_none [BEq α] {l : List (Σ a, β a)} {a : α} :
-    l.findKey? a = none ↔ l.containsKey a = false := by
-  rw [findKey?_eq_findEntry?, Option.map_eq_none', findEntry?_eq_none]
+theorem getKey?_eq_none [BEq α] {l : List (Σ a, β a)} {a : α} :
+    l.getKey? a = none ↔ l.containsKey a = false := by
+  rw [getKey?_eq_getEntry?, Option.map_eq_none', getEntry?_eq_none]
 
 @[simp]
-theorem findValue?_eq_none {β : Type v} [BEq α] {l : List ((_ : α) × β)} {a : α} :
-    l.findValue? a = none ↔ l.containsKey a = false := by
-  rw [findValue?_eq_findEntry?, Option.map_eq_none', findEntry?_eq_none]
+theorem getValue?_eq_none {β : Type v} [BEq α] {l : List ((_ : α) × β)} {a : α} :
+    l.getValue? a = none ↔ l.containsKey a = false := by
+  rw [getValue?_eq_getEntry?, Option.map_eq_none', getEntry?_eq_none]
 
 -- TODO
 @[simp] theorem Option.isSome_map (α : Type u) (β : Type v) (f : α → β) (o : Option α) :
     (o.map f).isSome = o.isSome := by
   cases o <;> simp
 
-theorem containsKey_eq_isSome_findValue? {β : Type v} [BEq α] {l : List ((_ : α) × β)} {a : α} :
-    l.containsKey a = (l.findValue? a).isSome := by
-  simp [containsKey_eq_isSome_findEntry?, findValue?_eq_findEntry?]
+theorem containsKey_eq_isSome_getValue? {β : Type v} [BEq α] {l : List ((_ : α) × β)} {a : α} :
+    l.containsKey a = (l.getValue? a).isSome := by
+  simp [containsKey_eq_isSome_getEntry?, getValue?_eq_getEntry?]
 
-theorem containsKey_eq_isSome_findKey? [BEq α] {l : List (Σ a, β a)} {a : α} :
-    l.containsKey a = (l.findKey? a).isSome := by
-  simp [containsKey_eq_isSome_findEntry?, findKey?_eq_findEntry?]
+theorem containsKey_eq_isSome_getKey? [BEq α] {l : List (Σ a, β a)} {a : α} :
+    l.containsKey a = (l.getKey? a).isSome := by
+  simp [containsKey_eq_isSome_getEntry?, getKey?_eq_getEntry?]
 
-theorem containsKey_eq_isSome_findValueCast? [BEq α] [LawfulBEq α] {l : List (Σ a, β a)} {a : α} :
-    l.containsKey a = (l.findValueCast? a).isSome := by
-  simp [containsKey_eq_isSome_findEntry?, findValueCast?_eq_findEntry?]
+theorem containsKey_eq_isSome_getValueCast? [BEq α] [LawfulBEq α] {l : List (Σ a, β a)} {a : α} :
+    l.containsKey a = (l.getValueCast? a).isSome := by
+  simp [containsKey_eq_isSome_getEntry?, getValueCast?_eq_getEntry?]
 
 theorem containsKey_eq_of_beq [BEq α] [PartialEquivBEq α] {l : List (Σ a, β a)} {a b : α} (h : a == b) :
     l.containsKey a = l.containsKey b := by
-  simp [containsKey_eq_isSome_findEntry?, findEntry?_eq_of_beq h]
+  simp [containsKey_eq_isSome_getEntry?, getEntry?_eq_of_beq h]
 
 theorem containsKey_of_beq [BEq α] [PartialEquivBEq α] {l : List (Σ a, β a)} {a b : α} (hla : l.containsKey a) (hab : a == b) :
     l.containsKey b := by
   rwa [← containsKey_eq_of_beq hab]
 
-def findEntry [BEq α] (l : List (Σ a, β a)) (a : α) (h : l.containsKey a) : Σ a, β a :=
-  (l.findEntry? a).get <| containsKey_eq_isSome_findEntry?.symm.trans h
+def getEntry [BEq α] (l : List (Σ a, β a)) (a : α) (h : l.containsKey a) : Σ a, β a :=
+  (l.getEntry? a).get <| containsKey_eq_isSome_getEntry?.symm.trans h
 
-theorem findEntry?_eq_some_findEntry [BEq α] {l : List (Σ a, β a)} {a : α} (h : l.containsKey a) :
-    l.findEntry? a = some (l.findEntry a h) := by
-  simp [findEntry]
+theorem getEntry?_eq_some_getEntry [BEq α] {l : List (Σ a, β a)} {a : α} (h : l.containsKey a) :
+    l.getEntry? a = some (l.getEntry a h) := by
+  simp [getEntry]
 
-theorem findEntry_eq_of_findEntry?_eq_some [BEq α] {l : List (Σ a, β a)} {k a : α} {v : β k}
-    (h : l.findEntry? a = some ⟨k, v⟩) {h'} : l.findEntry a h' = ⟨k, v⟩ := by
-  simp [findEntry, h]
+theorem getEntry_eq_of_getEntry?_eq_some [BEq α] {l : List (Σ a, β a)} {k a : α} {v : β k}
+    (h : l.getEntry? a = some ⟨k, v⟩) {h'} : l.getEntry a h' = ⟨k, v⟩ := by
+  simp [getEntry, h]
 
-theorem findEntry_cons_of_beq [BEq α] {l : List (Σ a, β a)} {k a : α} {v : β k} (h : k == a) :
-    (⟨k, v⟩ :: l).findEntry a (containsKey_cons_of_beq (v := v) h) = ⟨k, v⟩ := by
-  simp [findEntry, findEntry?_cons_of_true h]
+theorem getEntry_cons_of_beq [BEq α] {l : List (Σ a, β a)} {k a : α} {v : β k} (h : k == a) :
+    (⟨k, v⟩ :: l).getEntry a (containsKey_cons_of_beq (v := v) h) = ⟨k, v⟩ := by
+  simp [getEntry, getEntry?_cons_of_true h]
 
 @[simp]
-theorem findEntry_cons_self [BEq α] [ReflBEq α] {l : List (Σ a, β a)} {k : α} {v : β k} :
-    (⟨k, v⟩ :: l).findEntry k containsKey_cons_self = ⟨k, v⟩ :=
-  findEntry_cons_of_beq BEq.refl
+theorem getEntry_cons_self [BEq α] [ReflBEq α] {l : List (Σ a, β a)} {k : α} {v : β k} :
+    (⟨k, v⟩ :: l).getEntry k containsKey_cons_self = ⟨k, v⟩ :=
+  getEntry_cons_of_beq BEq.refl
 
-theorem findEntry_cons_of_false [BEq α] {l : List (Σ a, β a)} {k a : α} {v : β k} {h₁ : (⟨k, v⟩ :: l).containsKey a}
+theorem getEntry_cons_of_false [BEq α] {l : List (Σ a, β a)} {k a : α} {v : β k} {h₁ : (⟨k, v⟩ :: l).containsKey a}
     (h₂ : (k == a) = false) :
-    (⟨k, v⟩ :: l).findEntry a h₁ = l.findEntry a (containsKey_of_containsKey_cons (v := v) h₁ h₂) := by
-  simp [findEntry, findEntry?_cons_of_false h₂]
+    (⟨k, v⟩ :: l).getEntry a h₁ = l.getEntry a (containsKey_of_containsKey_cons (v := v) h₁ h₂) := by
+  simp [getEntry, getEntry?_cons_of_false h₂]
 
-def findKey [BEq α] (l : List (Σ a, β a)) (a : α) (h : l.containsKey a) : α :=
-  (l.findKey? a).get <| containsKey_eq_isSome_findKey?.symm.trans h
+def getKey [BEq α] (l : List (Σ a, β a)) (a : α) (h : l.containsKey a) : α :=
+  (l.getKey? a).get <| containsKey_eq_isSome_getKey?.symm.trans h
 
-theorem findKey?_eq_some_findKey [BEq α] {l : List (Σ a, β a)} {a : α} (h : l.containsKey a) :
-    l.findKey? a = some (l.findKey a h) := by
-  simp [findKey]
+theorem getKey?_eq_some_getKey [BEq α] {l : List (Σ a, β a)} {a : α} (h : l.containsKey a) :
+    l.getKey? a = some (l.getKey a h) := by
+  simp [getKey]
 
-theorem findKey_cons_of_beq [BEq α] {l : List (Σ a, β a)} {k a : α} {v : β k} (h : k == a) :
-    (⟨k, v⟩ :: l).findKey a (containsKey_cons_of_beq (v := v) h) = k := by
-  simp [findKey, findKey?_cons_of_true h]
+theorem getKey_cons_of_beq [BEq α] {l : List (Σ a, β a)} {k a : α} {v : β k} (h : k == a) :
+    (⟨k, v⟩ :: l).getKey a (containsKey_cons_of_beq (v := v) h) = k := by
+  simp [getKey, getKey?_cons_of_true h]
 
 @[simp]
-theorem findKey_cons_self [BEq α] [ReflBEq α] {l : List (Σ a, β a)} {k : α} {v : β k} :
-    (⟨k, v⟩ :: l).findKey k containsKey_cons_self = k :=
-  findKey_cons_of_beq BEq.refl
+theorem getKey_cons_self [BEq α] [ReflBEq α] {l : List (Σ a, β a)} {k : α} {v : β k} :
+    (⟨k, v⟩ :: l).getKey k containsKey_cons_self = k :=
+  getKey_cons_of_beq BEq.refl
 
-theorem findKey_cons_of_false [BEq α] {l : List (Σ a, β a)} {k a : α} {v : β k} {h₁ : (⟨k, v⟩ :: l).containsKey a}
-    (h₂ : (k == a) = false) : (⟨k, v⟩ :: l).findKey a h₁ = l.findKey a (containsKey_of_containsKey_cons (v := v) h₁ h₂) := by
-  simp [findKey, findKey?_cons_of_false h₂]
+theorem getKey_cons_of_false [BEq α] {l : List (Σ a, β a)} {k a : α} {v : β k} {h₁ : (⟨k, v⟩ :: l).containsKey a}
+    (h₂ : (k == a) = false) : (⟨k, v⟩ :: l).getKey a h₁ = l.getKey a (containsKey_of_containsKey_cons (v := v) h₁ h₂) := by
+  simp [getKey, getKey?_cons_of_false h₂]
 
-theorem findKey_beq [BEq α] {l : List (Σ a, β a)} {a : α} {h : l.containsKey a} : l.findKey a h == a := by
+theorem getKey_beq [BEq α] {l : List (Σ a, β a)} {a : α} {h : l.containsKey a} : l.getKey a h == a := by
   induction l using assoc_induction
   · simp at h
   · next k v t ih =>
     cases h' : k == a
-    · rw [findKey_cons_of_false h']
+    · rw [getKey_cons_of_false h']
       exact @ih (containsKey_of_containsKey_cons h h')
-    · rwa [findKey_cons_of_beq h']
+    · rwa [getKey_cons_of_beq h']
 
 section
 
 variable {β : Type v}
 
-def findValue [BEq α] (l : List ((_ : α) × β)) (a : α) (h : l.containsKey a) : β :=
-  (l.findValue? a).get <| containsKey_eq_isSome_findValue?.symm.trans h
+def getValue [BEq α] (l : List ((_ : α) × β)) (a : α) (h : l.containsKey a) : β :=
+  (l.getValue? a).get <| containsKey_eq_isSome_getValue?.symm.trans h
 
-theorem findValue?_eq_some_find [BEq α] {l : List ((_ : α) × β)} {a : α} (h : l.containsKey a) :
-    l.findValue? a = some (l.findValue a h) := by
-  simp [findValue]
+theorem getValue?_eq_some_get [BEq α] {l : List ((_ : α) × β)} {a : α} (h : l.containsKey a) :
+    l.getValue? a = some (l.getValue a h) := by
+  simp [getValue]
 
-theorem findValue_cons_of_beq [BEq α] {l : List ((_ : α) × β)} {k a : α} {v : β} (h : k == a) :
-    (⟨k, v⟩ :: l).findValue a (containsKey_cons_of_beq (k := k) (v := v) h) = v := by
-  simp [findValue, findValue?_cons_of_true h]
+theorem getValue_cons_of_beq [BEq α] {l : List ((_ : α) × β)} {k a : α} {v : β} (h : k == a) :
+    (⟨k, v⟩ :: l).getValue a (containsKey_cons_of_beq (k := k) (v := v) h) = v := by
+  simp [getValue, getValue?_cons_of_true h]
 
 @[simp]
-theorem findValue_cons_self [BEq α] [ReflBEq α] {l : List ((_ : α) × β)} {k : α} {v : β} :
-    (⟨k, v⟩ :: l).findValue k containsKey_cons_self = v :=
-  findValue_cons_of_beq BEq.refl
+theorem getValue_cons_self [BEq α] [ReflBEq α] {l : List ((_ : α) × β)} {k : α} {v : β} :
+    (⟨k, v⟩ :: l).getValue k containsKey_cons_self = v :=
+  getValue_cons_of_beq BEq.refl
 
-theorem findValue_cons_of_false [BEq α] {l : List ((_ : α) × β)} {k a : α} {v : β} {h₁ : (⟨k, v⟩ :: l).containsKey a}
-    (h₂ : (k == a) = false) : (⟨k, v⟩ :: l).findValue a h₁ = l.findValue a (containsKey_of_containsKey_cons (k := k) (v := v) h₁ h₂) := by
-  simp [findValue, findValue?_cons_of_false h₂]
+theorem getValue_cons_of_false [BEq α] {l : List ((_ : α) × β)} {k a : α} {v : β} {h₁ : (⟨k, v⟩ :: l).containsKey a}
+    (h₂ : (k == a) = false) : (⟨k, v⟩ :: l).getValue a h₁ = l.getValue a (containsKey_of_containsKey_cons (k := k) (v := v) h₁ h₂) := by
+  simp [getValue, getValue?_cons_of_false h₂]
 
 end
 
@@ -451,41 +451,41 @@ theorem isEmpty_replaceEntry [BEq α] {l : List (Σ a, β a)} {a : α} {b : β a
   · simp [replaceEntry_cons, cond_eq_if]
     split <;> simp
 
-theorem findEntry?_replaceEntry_of_containsKey_eq_false [BEq α] {l : List (Σ a, β a)} {k a : α} {b : β a}
-    (hl : l.containsKey a = false) : (l.replaceEntry a b).findEntry? k = l.findEntry? k := by
+theorem getEntry?_replaceEntry_of_containsKey_eq_false [BEq α] {l : List (Σ a, β a)} {k a : α} {b : β a}
+    (hl : l.containsKey a = false) : (l.replaceEntry a b).getEntry? k = l.getEntry? k := by
   rw [replaceEntry_of_containsKey_eq_false hl]
 
-theorem findEntry?_replaceEntry_of_false [BEq α] [PartialEquivBEq α] {l : List (Σ a, β a)} {k a : α} {b : β a}
-    (h : (k == a) = false) : (l.replaceEntry a b).findEntry? k = l.findEntry? k := by
+theorem getEntry?_replaceEntry_of_false [BEq α] [PartialEquivBEq α] {l : List (Σ a, β a)} {k a : α} {b : β a}
+    (h : (k == a) = false) : (l.replaceEntry a b).getEntry? k = l.getEntry? k := by
   induction l using assoc_induction
   · simp
   · next k' v' l ih =>
     cases h' : k' == a
-    · rw [replaceEntry_cons_of_false h', findEntry?_cons, findEntry?_cons, ih]
+    · rw [replaceEntry_cons_of_false h', getEntry?_cons, getEntry?_cons, ih]
     · rw [replaceEntry_cons_of_true h']
       have hk : (k' == k) = false := BEq.neq_of_beq_of_neq h' (BEq.symm_false h)
-      simp [findEntry?_cons_of_false (BEq.symm_false h), findEntry?_cons_of_false hk]
+      simp [getEntry?_cons_of_false (BEq.symm_false h), getEntry?_cons_of_false hk]
 
-theorem findEntry?_replaceEntry_of_true [BEq α] [PartialEquivBEq α] {l : List (Σ a, β a)} {k a : α} {b : β a} (hl : l.containsKey a = true)
-    (h : k == a) : (l.replaceEntry a b).findEntry? k = some ⟨a, b⟩ := by
+theorem getEntry?_replaceEntry_of_true [BEq α] [PartialEquivBEq α] {l : List (Σ a, β a)} {k a : α} {b : β a} (hl : l.containsKey a = true)
+    (h : k == a) : (l.replaceEntry a b).getEntry? k = some ⟨a, b⟩ := by
   induction l using assoc_induction
   · simp at hl
   · next k' v' l ih =>
     cases hk'a : k' == a
     · rw [replaceEntry_cons_of_false hk'a]
       have hk'k : (k' == k) = false := BEq.neq_of_neq_of_beq hk'a (BEq.symm h)
-      rw [findEntry?_cons_of_false hk'k]
+      rw [getEntry?_cons_of_false hk'k]
       exact ih (containsKey_of_containsKey_cons hl hk'a)
-    · rw [replaceEntry_cons_of_true hk'a, findEntry?_cons_of_true (BEq.symm h)]
+    · rw [replaceEntry_cons_of_true hk'a, getEntry?_cons_of_true (BEq.symm h)]
 
-theorem findEntry?_replaceEntry [BEq α] [PartialEquivBEq α] {l : List (Σ a, β a)} {k a : α} {b : β a} :
-    (l.replaceEntry a b).findEntry? k = bif l.containsKey a && k == a then some ⟨a, b⟩ else
-      l.findEntry? k := by
+theorem getEntry?_replaceEntry [BEq α] [PartialEquivBEq α] {l : List (Σ a, β a)} {k a : α} {b : β a} :
+    (l.replaceEntry a b).getEntry? k = bif l.containsKey a && k == a then some ⟨a, b⟩ else
+      l.getEntry? k := by
   cases hl : l.containsKey a
-  · simp [findEntry?_replaceEntry_of_containsKey_eq_false hl]
+  · simp [getEntry?_replaceEntry_of_containsKey_eq_false hl]
   · cases h : k == a
-    · simp [findEntry?_replaceEntry_of_false h]
-    · simp [findEntry?_replaceEntry_of_true hl h]
+    · simp [getEntry?_replaceEntry_of_false h]
+    · simp [getEntry?_replaceEntry_of_true hl h]
 
 @[simp]
 theorem length_replaceEntry [BEq α] {l : List (Σ a, β a)} {k : α} {v : β k} :
@@ -496,93 +496,93 @@ section
 
 variable {β : Type v}
 
-theorem findValue?_replaceEntry_of_containsKey_eq_false [BEq α] {l : List ((_ : α) × β)} {k a : α} {b : β}
-    (hl : l.containsKey a = false) : (l.replaceEntry a b).findValue? k = l.findValue? k := by
-  simp [findValue?_eq_findEntry?, findEntry?_replaceEntry_of_containsKey_eq_false hl]
+theorem getValue?_replaceEntry_of_containsKey_eq_false [BEq α] {l : List ((_ : α) × β)} {k a : α} {b : β}
+    (hl : l.containsKey a = false) : (l.replaceEntry a b).getValue? k = l.getValue? k := by
+  simp [getValue?_eq_getEntry?, getEntry?_replaceEntry_of_containsKey_eq_false hl]
 
-theorem findValue?_replaceEntry_of_false [BEq α] [PartialEquivBEq α] {l : List ((_ : α) × β)} {k a : α} {b : β}
-    (h : (k == a) = false) : (l.replaceEntry a b).findValue? k = l.findValue? k := by
-  simp [findValue?_eq_findEntry?, findEntry?_replaceEntry_of_false h]
+theorem getValue?_replaceEntry_of_false [BEq α] [PartialEquivBEq α] {l : List ((_ : α) × β)} {k a : α} {b : β}
+    (h : (k == a) = false) : (l.replaceEntry a b).getValue? k = l.getValue? k := by
+  simp [getValue?_eq_getEntry?, getEntry?_replaceEntry_of_false h]
 
-theorem findValue?_replaceEntry_of_true [BEq α] [PartialEquivBEq α] {l : List ((_ : α) × β)} {k a : α} {b : β}
-    (hl : l.containsKey a = true) (h : k == a) : (l.replaceEntry a b).findValue? k = some b := by
-  simp [findValue?_eq_findEntry?, findEntry?_replaceEntry_of_true hl h]
+theorem getValue?_replaceEntry_of_true [BEq α] [PartialEquivBEq α] {l : List ((_ : α) × β)} {k a : α} {b : β}
+    (hl : l.containsKey a = true) (h : k == a) : (l.replaceEntry a b).getValue? k = some b := by
+  simp [getValue?_eq_getEntry?, getEntry?_replaceEntry_of_true hl h]
 
 end
 
-theorem findKey?_replaceEntry_of_containsKey_eq_false [BEq α] {l : List (Σ a, β a)} {k a : α} {b : β a}
-    (hl : l.containsKey a = false) : (l.replaceEntry a b).findKey? k = l.findKey? k := by
-  simp [findKey?_eq_findEntry?, findEntry?_replaceEntry_of_containsKey_eq_false hl]
+theorem getKey?_replaceEntry_of_containsKey_eq_false [BEq α] {l : List (Σ a, β a)} {k a : α} {b : β a}
+    (hl : l.containsKey a = false) : (l.replaceEntry a b).getKey? k = l.getKey? k := by
+  simp [getKey?_eq_getEntry?, getEntry?_replaceEntry_of_containsKey_eq_false hl]
 
-theorem findKey?_replaceEntry_of_false [BEq α] [PartialEquivBEq α] {l : List (Σ a, β a)} {k a : α} {b : β a}
-    (h : (k == a) = false) : (l.replaceEntry a b).findKey? k = l.findKey? k := by
-  simp [findKey?_eq_findEntry?, findEntry?_replaceEntry_of_false h]
+theorem getKey?_replaceEntry_of_false [BEq α] [PartialEquivBEq α] {l : List (Σ a, β a)} {k a : α} {b : β a}
+    (h : (k == a) = false) : (l.replaceEntry a b).getKey? k = l.getKey? k := by
+  simp [getKey?_eq_getEntry?, getEntry?_replaceEntry_of_false h]
 
-theorem findKey?_replaceEntry_of_true [BEq α] [PartialEquivBEq α] {l : List (Σ a, β a)} {k a : α} {b : β a}
-    (hl : l.containsKey a = true) (h : (k == a)) : (l.replaceEntry a b).findKey? k = some a := by
-  simp [findKey?_eq_findEntry?, findEntry?_replaceEntry_of_true hl h]
+theorem getKey?_replaceEntry_of_true [BEq α] [PartialEquivBEq α] {l : List (Σ a, β a)} {k a : α} {b : β a}
+    (hl : l.containsKey a = true) (h : (k == a)) : (l.replaceEntry a b).getKey? k = some a := by
+  simp [getKey?_eq_getEntry?, getEntry?_replaceEntry_of_true hl h]
 
-theorem findKey?_replaceEntry [BEq α] [PartialEquivBEq α] {l : List (Σ a, β a)} {k a : α} {b : β a} :
-    (l.replaceEntry a b).findKey? k = bif l.containsKey a && k == a then some a else l.findKey? k := by
+theorem getKey?_replaceEntry [BEq α] [PartialEquivBEq α] {l : List (Σ a, β a)} {k a : α} {b : β a} :
+    (l.replaceEntry a b).getKey? k = bif l.containsKey a && k == a then some a else l.getKey? k := by
   cases hl : l.containsKey a
-  · simp [findKey?_replaceEntry_of_containsKey_eq_false hl]
+  · simp [getKey?_replaceEntry_of_containsKey_eq_false hl]
   · cases h : k == a
-    · simp [findKey?_replaceEntry_of_false h]
-    · simp [findKey?_replaceEntry_of_true hl h]
+    · simp [getKey?_replaceEntry_of_false h]
+    · simp [getKey?_replaceEntry_of_true hl h]
 
 @[simp]
 theorem containsKey_replaceEntry [BEq α] [PartialEquivBEq α] {l : List (Σ a, β a)} {k a : α} {b : β a} :
     (l.replaceEntry a b).containsKey k = l.containsKey k := by
   cases h : l.containsKey a && k == a
-  · rw [containsKey_eq_isSome_findKey?, findKey?_replaceEntry, h, cond_false, containsKey_eq_isSome_findKey?]
-  · rw [containsKey_eq_isSome_findKey?, findKey?_replaceEntry, h, cond_true, Option.isSome_some, Eq.comm]
+  · rw [containsKey_eq_isSome_getKey?, getKey?_replaceEntry, h, cond_false, containsKey_eq_isSome_getKey?]
+  · rw [containsKey_eq_isSome_getKey?, getKey?_replaceEntry, h, cond_true, Option.isSome_some, Eq.comm]
     rw [Bool.and_eq_true] at h
     exact containsKey_of_beq h.1 (BEq.symm h.2)
 
-def eraseKey [BEq α] (a : α) : List (Σ a, β a) → List (Σ a, β a)
+def removeKey [BEq α] (a : α) : List (Σ a, β a) → List (Σ a, β a)
   | nil => nil
-  | ⟨k, v⟩ :: l => bif k == a then l else ⟨k, v⟩ :: l.eraseKey a
+  | ⟨k, v⟩ :: l => bif k == a then l else ⟨k, v⟩ :: l.removeKey a
 
-@[simp] theorem eraseKey_nil [BEq α] {a : α} : (nil : List (Σ a, β a)).eraseKey a = nil := rfl
-theorem eraseKey_cons [BEq α] {l : List (Σ a, β a)} {k a : α} {v : β k} :
-    (⟨k, v⟩ :: l).eraseKey a = bif k == a then l else ⟨k, v⟩ :: l.eraseKey a := rfl
+@[simp] theorem removeKey_nil [BEq α] {a : α} : (nil : List (Σ a, β a)).removeKey a = nil := rfl
+theorem removeKey_cons [BEq α] {l : List (Σ a, β a)} {k a : α} {v : β k} :
+    (⟨k, v⟩ :: l).removeKey a = bif k == a then l else ⟨k, v⟩ :: l.removeKey a := rfl
 
-theorem eraseKey_cons_of_beq [BEq α] {l : List (Σ a, β a)} {k a : α} {v : β k} (h : k == a) :
-    (⟨k, v⟩ :: l).eraseKey a = l :=
-  by simp [eraseKey_cons, h]
+theorem removeKey_cons_of_beq [BEq α] {l : List (Σ a, β a)} {k a : α} {v : β k} (h : k == a) :
+    (⟨k, v⟩ :: l).removeKey a = l :=
+  by simp [removeKey_cons, h]
 
 @[simp]
-theorem eraseKey_cons_self [BEq α] [ReflBEq α] {l : List (Σ a, β a)} {k : α} {v : β k} :
-    (⟨k, v⟩ :: l).eraseKey k = l :=
-  eraseKey_cons_of_beq BEq.refl
+theorem removeKey_cons_self [BEq α] [ReflBEq α] {l : List (Σ a, β a)} {k : α} {v : β k} :
+    (⟨k, v⟩ :: l).removeKey k = l :=
+  removeKey_cons_of_beq BEq.refl
 
-theorem eraseKey_cons_of_false [BEq α] {l : List (Σ a, β a)} {k a : α} {v : β k} (h : (k == a) = false) :
-    (⟨k, v⟩ :: l).eraseKey a = ⟨k, v⟩ :: l.eraseKey a := by
-  simp [eraseKey_cons, h]
+theorem removeKey_cons_of_false [BEq α] {l : List (Σ a, β a)} {k a : α} {v : β k} (h : (k == a) = false) :
+    (⟨k, v⟩ :: l).removeKey a = ⟨k, v⟩ :: l.removeKey a := by
+  simp [removeKey_cons, h]
 
-theorem eraseKey_of_containsKey_eq_false [BEq α] {l : List (Σ a, β a)} {k : α} (h : l.containsKey k = false) :
-    l.eraseKey k = l := by
+theorem removeKey_of_containsKey_eq_false [BEq α] {l : List (Σ a, β a)} {k : α} (h : l.containsKey k = false) :
+    l.removeKey k = l := by
   induction l using assoc_induction
   · simp
   · next k' v' t ih =>
     simp only [containsKey_cons, Bool.or_eq_false_iff] at h
-    rw [eraseKey_cons_of_false h.1, ih h.2]
+    rw [removeKey_cons_of_false h.1, ih h.2]
 
-theorem sublist_eraseKey [BEq α] {l : List (Σ a, β a)} {k : α} : (l.eraseKey k).Sublist l := by
+theorem sublist_removeKey [BEq α] {l : List (Σ a, β a)} {k : α} : (l.removeKey k).Sublist l := by
   induction l using assoc_induction
   · simp
   · next k' v' t ih =>
-    rw [eraseKey_cons]
+    rw [removeKey_cons]
     cases k' == k
     · simpa
     · simp
 
-theorem length_eraseKey [BEq α] {l : List (Σ a, β a)} {k : α} :
-    (l.eraseKey k).length = bif l.containsKey k then l.length - 1 else l.length := by
+theorem length_removeKey [BEq α] {l : List (Σ a, β a)} {k : α} :
+    (l.removeKey k).length = bif l.containsKey k then l.length - 1 else l.length := by
   induction l using assoc_induction
   · simp
   · next k' v' t ih =>
-    rw [eraseKey_cons, containsKey_cons]
+    rw [removeKey_cons, containsKey_cons]
     cases k' == k
     · rw [cond_false, Bool.false_or, length_cons, ih]
       cases h : containsKey k t
@@ -594,7 +594,7 @@ theorem length_eraseKey [BEq α] {l : List (Σ a, β a)} {k : α} :
         · simp
     · simp
 
--- TODO: eraseKey+replaceEntry
+-- TODO: removeKey+replaceEntry
 
 @[simp] theorem keys_nil : ([] : List (Σ a, β a)).keys = [] := rfl
 @[simp] theorem keys_cons {l : List (Σ a, β a)} {k : α} {v : β k} : (⟨k, v⟩ :: l).keys = k :: l.keys := rfl
@@ -676,19 +676,19 @@ theorem DistinctKeys.cons [BEq α] [PartialEquivBEq α] {l : List (Σ a, β a)} 
     l.DistinctKeys → (⟨k, v⟩ :: l).DistinctKeys :=
   fun h' => distinctKeys_cons_iff.mpr ⟨h', h⟩
 
-theorem mem_iff_findEntry?_eq_some [BEq α] [EquivBEq α] {l : List (Σ a, β a)} {p : Σ a, β a} (h : l.DistinctKeys) :
-    p ∈ l ↔ l.findEntry? p.1 = some p := by
+theorem mem_iff_getEntry?_eq_some [BEq α] [EquivBEq α] {l : List (Σ a, β a)} {p : Σ a, β a} (h : l.DistinctKeys) :
+    p ∈ l ↔ l.getEntry? p.1 = some p := by
   induction l using assoc_induction
   · simp_all
   · next k v t ih =>
-    simp only [mem_cons, findEntry?_cons, ih h.tail]
+    simp only [mem_cons, getEntry?_cons, ih h.tail]
     refine ⟨?_, ?_⟩
     · rintro (rfl|hk)
       · simp
       · suffices (k == p.fst) = false by simp_all
         refine Bool.eq_false_iff.2 fun hcon => Bool.false_ne_true ?_
         rw [← h.containsKey_eq_false, containsKey_eq_of_beq hcon,
-          containsKey_eq_isSome_findEntry?, hk, Option.isSome_some]
+          containsKey_eq_isSome_getEntry?, hk, Option.isSome_some]
     · cases k == p.fst
       · rw [cond_false]
         exact Or.inr
@@ -704,9 +704,9 @@ variable {β : Type v}
 theorem values_eq_map {l : List ((_ : α) × β)} : l.values = l.map (·.2) := by
   induction l using assoc_induction <;> simp_all
 
-theorem mem_values_iff_exists_findValue?_eq_some [BEq α] [EquivBEq α] {l : List ((_ : α) × β)} {v : β} (h : l.DistinctKeys) :
-    v ∈ l.values ↔ ∃ k, l.findValue? k = some v := by
-  simp only [values_eq_map, List.mem_map, mem_iff_findEntry?_eq_some h, findValue?_eq_findEntry?]
+theorem mem_values_iff_exists_getValue?_eq_some [BEq α] [EquivBEq α] {l : List ((_ : α) × β)} {v : β} (h : l.DistinctKeys) :
+    v ∈ l.values ↔ ∃ k, l.getValue? k = some v := by
+  simp only [values_eq_map, List.mem_map, mem_iff_getEntry?_eq_some h, getValue?_eq_getEntry?]
   refine ⟨?_, ?_⟩
   · rintro ⟨p, hp, rfl⟩
     exact ⟨p.1, by simp_all⟩
@@ -714,7 +714,7 @@ theorem mem_values_iff_exists_findValue?_eq_some [BEq α] [EquivBEq α] {l : Lis
     simp only [Option.map_eq_some'] at hk
     rcases hk with ⟨a, ha, rfl⟩
     refine ⟨a, ⟨?_, rfl⟩⟩
-    rw [findEntry?_eq_of_beq (findEntry?_eq_some ha), ha]
+    rw [getEntry?_eq_of_beq (getEntry?_eq_some ha), ha]
 
 end
 
@@ -764,31 +764,31 @@ section
 
 variable {β : Type v}
 
-theorem findValue?_insertEntry_of_beq [BEq α] [PartialEquivBEq α] {l : List ((_ : α) × β)} {k a : α} {v : β} (h : k == a) :
-    (l.insertEntry k v).findValue? a = some v := by
+theorem getValue?_insertEntry_of_beq [BEq α] [PartialEquivBEq α] {l : List ((_ : α) × β)} {k a : α} {v : β} (h : k == a) :
+    (l.insertEntry k v).getValue? a = some v := by
   cases h' : l.containsKey k
-  · rw [insertEntry_of_containsKey_eq_false h', findValue?_cons_of_true h]
-  · rw [insertEntry_of_containsKey h', findValue?_replaceEntry_of_true h' (BEq.symm h)]
+  · rw [insertEntry_of_containsKey_eq_false h', getValue?_cons_of_true h]
+  · rw [insertEntry_of_containsKey h', getValue?_replaceEntry_of_true h' (BEq.symm h)]
 
-theorem findValue?_insertEntry_of_self [BEq α] [EquivBEq α] {l : List ((_ : α) × β)} {k : α} {v : β} :
-    (l.insertEntry k v).findValue? k = some v :=
-  findValue?_insertEntry_of_beq BEq.refl
+theorem getValue?_insertEntry_of_self [BEq α] [EquivBEq α] {l : List ((_ : α) × β)} {k : α} {v : β} :
+    (l.insertEntry k v).getValue? k = some v :=
+  getValue?_insertEntry_of_beq BEq.refl
 
-theorem findValue?_insertEntry_of_false [BEq α] [PartialEquivBEq α] {l : List ((_ : α) × β)} {k a : α} {v : β} (h : (k == a) = false) :
-    (l.insertEntry k v).findValue? a = l.findValue? a := by
+theorem getValue?_insertEntry_of_false [BEq α] [PartialEquivBEq α] {l : List ((_ : α) × β)} {k a : α} {v : β} (h : (k == a) = false) :
+    (l.insertEntry k v).getValue? a = l.getValue? a := by
   cases h' : l.containsKey k
-  · rw [insertEntry_of_containsKey_eq_false h', findValue?_cons_of_false h]
-  · rw [insertEntry_of_containsKey h', findValue?_replaceEntry_of_false (BEq.symm_false h)]
+  · rw [insertEntry_of_containsKey_eq_false h', getValue?_cons_of_false h]
+  · rw [insertEntry_of_containsKey h', getValue?_replaceEntry_of_false (BEq.symm_false h)]
 
-theorem findValue?_insertEntry [BEq α] [PartialEquivBEq α] {l : List ((_ : α) × β)} {k a : α} {v : β} :
-    (l.insertEntry k v).findValue? a = bif k == a then some v else l.findValue? a := by
+theorem getValue?_insertEntry [BEq α] [PartialEquivBEq α] {l : List ((_ : α) × β)} {k a : α} {v : β} :
+    (l.insertEntry k v).getValue? a = bif k == a then some v else l.getValue? a := by
   cases h : k == a
-  · simp [findValue?_insertEntry_of_false h, h]
-  · simp [findValue?_insertEntry_of_beq h, h]
+  · simp [getValue?_insertEntry_of_false h, h]
+  · simp [getValue?_insertEntry_of_beq h, h]
 
 theorem mem_values_insertEntry [BEq α] [EquivBEq α] {l : List ((_ : α) × β)} {a : α} {b v : β}
-    (h : l.DistinctKeys) : v ∈ (l.insertEntry a b).values ↔ b = v ∨ ∃ k, (a == k) = false ∧ l.findValue? k = some v := by
-  simp only [mem_values_iff_exists_findValue?_eq_some h.insertEntry, findValue?_insertEntry, cond_eq_if]
+    (h : l.DistinctKeys) : v ∈ (l.insertEntry a b).values ↔ b = v ∨ ∃ k, (a == k) = false ∧ l.getValue? k = some v := by
+  simp only [mem_values_iff_exists_getValue?_eq_some h.insertEntry, getValue?_insertEntry, cond_eq_if]
   refine ⟨?_, ?_⟩
   · simp only [forall_exists_index]
     intro a'
@@ -819,33 +819,33 @@ theorem mem_values_insertEntry_self [BEq α] [ReflBEq α] {l : List ((_ : α) ×
 end
 
 -- TODO: Unify order in `bif k == a` vs. `bif a == k`.
-theorem findKey?_insertEntry_of_containsKey [BEq α] [PartialEquivBEq α] {l : List (Σ a, β a)} {k a : α} {v : β k}
-    (h : l.containsKey k) : (l.insertEntry k v).findKey? a = bif k == a then some k else l.findKey? a := by
-  simp [insertEntry_of_containsKey h, findKey?_replaceEntry, h, BEq.comm]
+theorem getKey?_insertEntry_of_containsKey [BEq α] [PartialEquivBEq α] {l : List (Σ a, β a)} {k a : α} {v : β k}
+    (h : l.containsKey k) : (l.insertEntry k v).getKey? a = bif k == a then some k else l.getKey? a := by
+  simp [insertEntry_of_containsKey h, getKey?_replaceEntry, h, BEq.comm]
 
-theorem findKey?_insertEntry_of_containsKey_eq_false [BEq α] [PartialEquivBEq α] {l : List (Σ a, β a)} {k a : α} {v : β k}
+theorem getKey?_insertEntry_of_containsKey_eq_false [BEq α] [PartialEquivBEq α] {l : List (Σ a, β a)} {k a : α} {v : β k}
     (hl : (l.containsKey k) = false) :
-    (l.insertEntry k v).findKey? a = bif k == a then some k else l.findKey? a := by
-  simp [insertEntry_of_containsKey_eq_false hl, findKey?_cons]
+    (l.insertEntry k v).getKey? a = bif k == a then some k else l.getKey? a := by
+  simp [insertEntry_of_containsKey_eq_false hl, getKey?_cons]
 
-theorem findKey?_insertEntry [BEq α] [PartialEquivBEq α] {l : List (Σ a, β a)} {k a : α} {v : β k} :
-    (l.insertEntry k v).findKey? a = bif k == a then some k else l.findKey? a := by
+theorem getKey?_insertEntry [BEq α] [PartialEquivBEq α] {l : List (Σ a, β a)} {k a : α} {v : β k} :
+    (l.insertEntry k v).getKey? a = bif k == a then some k else l.getKey? a := by
   cases hl : l.containsKey k
-  · simp [findKey?_insertEntry_of_containsKey_eq_false hl, hl]
-  · simp [findKey?_insertEntry_of_containsKey hl]
+  · simp [getKey?_insertEntry_of_containsKey_eq_false hl, hl]
+  · simp [getKey?_insertEntry_of_containsKey hl]
 
-theorem findEntry?_insertEntry [BEq α] [PartialEquivBEq α] {l : List (Σ a, β a)} {k a : α} {v : β k} :
-    (l.insertEntry k v).findEntry? a = bif k == a then some ⟨k, v⟩ else l.findEntry? a := by
+theorem getEntry?_insertEntry [BEq α] [PartialEquivBEq α] {l : List (Σ a, β a)} {k a : α} {v : β k} :
+    (l.insertEntry k v).getEntry? a = bif k == a then some ⟨k, v⟩ else l.getEntry? a := by
   cases hl : l.containsKey k
-  · rw [insertEntry_of_containsKey_eq_false hl, findEntry?_cons]
-  · rw [insertEntry_of_containsKey hl, findEntry?_replaceEntry, hl, Bool.true_and, BEq.comm]
+  · rw [insertEntry_of_containsKey_eq_false hl, getEntry?_cons]
+  · rw [insertEntry_of_containsKey hl, getEntry?_replaceEntry, hl, Bool.true_and, BEq.comm]
 
--- TODO: findEntry?_insertEntry_of_beq, findEntry?_insertEntry_of_beq_eq_false
+-- TODO: getEntry?_insertEntry_of_beq, getEntry?_insertEntry_of_beq_eq_false
 
 @[simp]
 theorem containsKey_insertEntry [BEq α] [PartialEquivBEq α] {l : List (Σ a, β a)} {k a : α} {v : β k} :
     (l.insertEntry k v).containsKey a = ((k == a) || l.containsKey a) := by
-  rw [containsKey_eq_isSome_findKey?, containsKey_eq_isSome_findKey?, findKey?_insertEntry]
+  rw [containsKey_eq_isSome_getKey?, containsKey_eq_isSome_getKey?, getKey?_insertEntry]
   cases k == a
   · simp
   · simp
@@ -860,54 +860,54 @@ theorem containsKey_insertEntry_self [BEq α] [EquivBEq α] {l : List (Σ a, β 
   containsKey_insertEntry_of_beq BEq.refl
 
 @[simp]
-theorem keys_eraseKey [BEq α] [PartialEquivBEq α] {l : List (Σ a, β a)} {k : α} :
-    (l.eraseKey k).keys = l.keys.erase k := by
+theorem keys_removeKey [BEq α] [PartialEquivBEq α] {l : List (Σ a, β a)} {k : α} :
+    (l.removeKey k).keys = l.keys.erase k := by
   induction l using assoc_induction
   · rfl
   · next k' v' l ih =>
-    simp only [eraseKey_cons, keys_cons, List.erase_cons]
+    simp only [removeKey_cons, keys_cons, List.erase_cons]
     cases k' == k
     · simp [ih]
     · simp [ih]
 
-theorem DistinctKeys.eraseKey [BEq α] [PartialEquivBEq α] {l : List (Σ a, β a)} {k : α} : l.DistinctKeys → (l.eraseKey k).DistinctKeys := by
+theorem DistinctKeys.removeKey [BEq α] [PartialEquivBEq α] {l : List (Σ a, β a)} {k : α} : l.DistinctKeys → (l.removeKey k).DistinctKeys := by
   apply distinctKeys_of_sublist_keys (by simpa using List.erase_sublist _ _)
 
-theorem findEntry?_eraseKey_self [BEq α] [PartialEquivBEq α] {l : List (Σ a, β a)} {k : α} (h : l.DistinctKeys) :
-    (l.eraseKey k).findEntry? k = none := by
+theorem getEntry?_removeKey_self [BEq α] [PartialEquivBEq α] {l : List (Σ a, β a)} {k : α} (h : l.DistinctKeys) :
+    (l.removeKey k).getEntry? k = none := by
   induction l using assoc_induction
   · simp
   · next k' v' t ih =>
     cases h' : k' == k
-    · rw [eraseKey_cons_of_false h', findEntry?_cons_of_false h']
+    · rw [removeKey_cons_of_false h', getEntry?_cons_of_false h']
       exact ih h.tail
-    · rw [eraseKey_cons_of_beq h', ← Option.not_isSome_iff_eq_none, Bool.not_eq_true,
-        ← containsKey_eq_isSome_findEntry?, ← containsKey_eq_of_beq h']
+    · rw [removeKey_cons_of_beq h', ← Option.not_isSome_iff_eq_none, Bool.not_eq_true,
+        ← containsKey_eq_isSome_getEntry?, ← containsKey_eq_of_beq h']
       exact h.containsKey_eq_false
 
-theorem findEntry?_eraseKey_of_beq [BEq α] [PartialEquivBEq α] {l : List (Σ a, β a)} {k a : α} (hl : l.DistinctKeys)
-    (hka : k == a) : (l.eraseKey k).findEntry? a = none := by
-  rw [← findEntry?_eq_of_beq hka, findEntry?_eraseKey_self hl]
+theorem getEntry?_removeKey_of_beq [BEq α] [PartialEquivBEq α] {l : List (Σ a, β a)} {k a : α} (hl : l.DistinctKeys)
+    (hka : k == a) : (l.removeKey k).getEntry? a = none := by
+  rw [← getEntry?_eq_of_beq hka, getEntry?_removeKey_self hl]
 
-theorem findEntry?_eraseKey_of_false [BEq α] [PartialEquivBEq α] {l : List (Σ a, β a)} {k a : α}
-    (hka : (k == a) = false) : (l.eraseKey k).findEntry? a = l.findEntry? a := by
+theorem getEntry?_removeKey_of_false [BEq α] [PartialEquivBEq α] {l : List (Σ a, β a)} {k a : α}
+    (hka : (k == a) = false) : (l.removeKey k).getEntry? a = l.getEntry? a := by
   induction l using assoc_induction
   · simp
   · next k' v' t ih =>
     cases h' : k' == k
-    · rw [eraseKey_cons_of_false h']
+    · rw [removeKey_cons_of_false h']
       cases h'' : k' == a
-      · rw [findEntry?_cons_of_false h'', ih, findEntry?_cons_of_false h'']
-      · rw [findEntry?_cons_of_true h'', findEntry?_cons_of_true h'']
-    · rw [eraseKey_cons_of_beq h']
+      · rw [getEntry?_cons_of_false h'', ih, getEntry?_cons_of_false h'']
+      · rw [getEntry?_cons_of_true h'', getEntry?_cons_of_true h'']
+    · rw [removeKey_cons_of_beq h']
       have hx : (k' == a) = false := BEq.neq_of_beq_of_neq h' hka
-      rw [findEntry?_cons_of_false hx]
+      rw [getEntry?_cons_of_false hx]
 
-theorem findEntry?_eraseKey [BEq α] [PartialEquivBEq α] {l : List (Σ a, β a)} {k a : α} (hl : l.DistinctKeys) :
-    (l.eraseKey k).findEntry? a = bif k == a then none else l.findEntry? a := by
+theorem getEntry?_removeKey [BEq α] [PartialEquivBEq α] {l : List (Σ a, β a)} {k a : α} (hl : l.DistinctKeys) :
+    (l.removeKey k).getEntry? a = bif k == a then none else l.getEntry? a := by
   cases h : k == a
-  · simp [findEntry?_eraseKey_of_false h, h]
-  · simp [findEntry?_eraseKey_of_beq hl h, h]
+  · simp [getEntry?_removeKey_of_false h, h]
+  · simp [getEntry?_removeKey_of_beq hl h, h]
 
 theorem keys_filterMap [BEq α] {l : List (Σ a, β a)} {f : (a : α) → β a → Option (γ a)} :
     (l.filterMap fun p => (f p.1 p.2).map (⟨p.1, ·⟩)).keys = (l.filter fun p => (f p.1 p.2).isSome).keys := by
@@ -938,75 +938,75 @@ section
 variable {β : Type v}
 
 -- TODO
-theorem findValue?_eraseKey_self [BEq α] [PartialEquivBEq α] {l : List ((_ : α) × β)} {k : α} (h : l.DistinctKeys) :
-    (l.eraseKey k).findValue? k = none := by
-  simp [findValue?_eq_findEntry?, findEntry?_eraseKey_self h]
+theorem getValue?_removeKey_self [BEq α] [PartialEquivBEq α] {l : List ((_ : α) × β)} {k : α} (h : l.DistinctKeys) :
+    (l.removeKey k).getValue? k = none := by
+  simp [getValue?_eq_getEntry?, getEntry?_removeKey_self h]
 
-theorem findValue?_eraseKey_of_beq [BEq α] [PartialEquivBEq α] {l : List ((_ : α) × β)} {k a : α} (hl : l.DistinctKeys)
-    (hka : k == a) : (l.eraseKey k).findValue? a = none := by
-  simp [findValue?_eq_findEntry?, findEntry?_eraseKey_of_beq hl hka]
+theorem getValue?_removeKey_of_beq [BEq α] [PartialEquivBEq α] {l : List ((_ : α) × β)} {k a : α} (hl : l.DistinctKeys)
+    (hka : k == a) : (l.removeKey k).getValue? a = none := by
+  simp [getValue?_eq_getEntry?, getEntry?_removeKey_of_beq hl hka]
 
-theorem findValue?_eraseKey_of_false [BEq α] [PartialEquivBEq α] {l : List ((_ : α) × β)} {k a : α}
-    (hka : (k == a) = false) : (l.eraseKey k).findValue? a = l.findValue? a := by
-  simp [findValue?_eq_findEntry?, findEntry?_eraseKey_of_false hka]
+theorem getValue?_removeKey_of_false [BEq α] [PartialEquivBEq α] {l : List ((_ : α) × β)} {k a : α}
+    (hka : (k == a) = false) : (l.removeKey k).getValue? a = l.getValue? a := by
+  simp [getValue?_eq_getEntry?, getEntry?_removeKey_of_false hka]
 
-theorem findValue?_eraseKey [BEq α] [PartialEquivBEq α] {l : List ((_ : α) × β)} {k a : α} (hl : l.DistinctKeys) :
-    (l.eraseKey k).findValue? a = bif k == a then none else l.findValue? a := by
-  simp [findValue?_eq_findEntry?, findEntry?_eraseKey hl, apply_bif (Option.map _)]
+theorem getValue?_removeKey [BEq α] [PartialEquivBEq α] {l : List ((_ : α) × β)} {k a : α} (hl : l.DistinctKeys) :
+    (l.removeKey k).getValue? a = bif k == a then none else l.getValue? a := by
+  simp [getValue?_eq_getEntry?, getEntry?_removeKey hl, apply_bif (Option.map _)]
 
 end
 
-theorem findKey?_eraseKey_self [BEq α] [PartialEquivBEq α] {l : List (Σ a, β a)} {k : α} (h : l.DistinctKeys) :
-    (l.eraseKey k).findKey? k = none := by
-  simp [findKey?_eq_findEntry?, findEntry?_eraseKey_self h]
+theorem getKey?_removeKey_self [BEq α] [PartialEquivBEq α] {l : List (Σ a, β a)} {k : α} (h : l.DistinctKeys) :
+    (l.removeKey k).getKey? k = none := by
+  simp [getKey?_eq_getEntry?, getEntry?_removeKey_self h]
 
-theorem findKey?_eraseKey_of_beq [BEq α] [PartialEquivBEq α] {l : List (Σ a, β a)} {k a : α} (hl : l.DistinctKeys)
-    (hka : k == a) : (l.eraseKey k).findKey? a = none := by
-  simp [findKey?_eq_findEntry?, findEntry?_eraseKey_of_beq hl hka]
+theorem getKey?_removeKey_of_beq [BEq α] [PartialEquivBEq α] {l : List (Σ a, β a)} {k a : α} (hl : l.DistinctKeys)
+    (hka : k == a) : (l.removeKey k).getKey? a = none := by
+  simp [getKey?_eq_getEntry?, getEntry?_removeKey_of_beq hl hka]
 
-theorem findKey?_eraseKey_of_false [BEq α] [PartialEquivBEq α] {l : List (Σ a, β a)} {k a : α}
-    (hka : (k == a) = false) : (l.eraseKey k).findKey? a = l.findKey? a := by
-  simp [findKey?_eq_findEntry?, findEntry?_eraseKey_of_false hka]
+theorem getKey?_removeKey_of_false [BEq α] [PartialEquivBEq α] {l : List (Σ a, β a)} {k a : α}
+    (hka : (k == a) = false) : (l.removeKey k).getKey? a = l.getKey? a := by
+  simp [getKey?_eq_getEntry?, getEntry?_removeKey_of_false hka]
 
-theorem findKey?_eraseKey [BEq α] [PartialEquivBEq α] {l : List (Σ a, β a)} {k a : α} (hl : l.DistinctKeys) :
-    (l.eraseKey k).findKey? a = bif k == a then none else l.findKey? a := by
-  simp [findKey?_eq_findEntry?, findEntry?_eraseKey hl, apply_bif (Option.map _)]
+theorem getKey?_removeKey [BEq α] [PartialEquivBEq α] {l : List (Σ a, β a)} {k a : α} (hl : l.DistinctKeys) :
+    (l.removeKey k).getKey? a = bif k == a then none else l.getKey? a := by
+  simp [getKey?_eq_getEntry?, getEntry?_removeKey hl, apply_bif (Option.map _)]
 
-theorem containsKey_eraseKey_self [BEq α] [PartialEquivBEq α] {l : List (Σ a, β a)} {k : α} (h : l.DistinctKeys) :
-    (l.eraseKey k).containsKey k = false := by
-  simp [containsKey_eq_isSome_findEntry?, findEntry?_eraseKey_self h]
+theorem containsKey_removeKey_self [BEq α] [PartialEquivBEq α] {l : List (Σ a, β a)} {k : α} (h : l.DistinctKeys) :
+    (l.removeKey k).containsKey k = false := by
+  simp [containsKey_eq_isSome_getEntry?, getEntry?_removeKey_self h]
 
-theorem containsKey_eraseKey_of_beq [BEq α] [PartialEquivBEq α] {l : List (Σ a, β a)} {k a : α} (hl : l.DistinctKeys)
-    (hka : k == a) : (l.eraseKey k).containsKey a = false := by
-  rw [← containsKey_eq_of_beq hka, containsKey_eraseKey_self hl]
+theorem containsKey_removeKey_of_beq [BEq α] [PartialEquivBEq α] {l : List (Σ a, β a)} {k a : α} (hl : l.DistinctKeys)
+    (hka : k == a) : (l.removeKey k).containsKey a = false := by
+  rw [← containsKey_eq_of_beq hka, containsKey_removeKey_self hl]
 
-theorem containsKey_eraseKey_of_false [BEq α] [PartialEquivBEq α] {l : List (Σ a, β a)} {k a : α}
-    (hka : (k == a) = false) : (l.eraseKey k).containsKey a = l.containsKey a := by
-  simp [containsKey_eq_isSome_findEntry?, findEntry?_eraseKey_of_false hka]
+theorem containsKey_removeKey_of_false [BEq α] [PartialEquivBEq α] {l : List (Σ a, β a)} {k a : α}
+    (hka : (k == a) = false) : (l.removeKey k).containsKey a = l.containsKey a := by
+  simp [containsKey_eq_isSome_getEntry?, getEntry?_removeKey_of_false hka]
 
 -- TODO: this should probably be something like (!(k == a)) && l.containsKey a
-theorem containsKey_eraseKey [BEq α] [PartialEquivBEq α] {l : List (Σ a, β a)} {k a : α} (hl : l.DistinctKeys) :
-    (l.eraseKey k).containsKey a = bif k == a then false else l.containsKey a := by
-  simp [containsKey_eq_isSome_findEntry?, findEntry?_eraseKey hl, apply_bif Option.isSome]
+theorem containsKey_removeKey [BEq α] [PartialEquivBEq α] {l : List (Σ a, β a)} {k a : α} (hl : l.DistinctKeys) :
+    (l.removeKey k).containsKey a = bif k == a then false else l.containsKey a := by
+  simp [containsKey_eq_isSome_getEntry?, getEntry?_removeKey hl, apply_bif Option.isSome]
 
 -- TODO: Technically this should be true without assuming l.DistinctKeys
-theorem containsKey_of_containsKey_eraseKey [BEq α] [PartialEquivBEq α] {l : List (Σ a, β a)} {k a : α} (hl : l.DistinctKeys)
-    (h : (l.eraseKey k).containsKey a) : l.containsKey a := by
+theorem containsKey_of_containsKey_removeKey [BEq α] [PartialEquivBEq α] {l : List (Σ a, β a)} {k a : α} (hl : l.DistinctKeys)
+    (h : (l.removeKey k).containsKey a) : l.containsKey a := by
   cases hka : k == a
-  · rwa [containsKey_eraseKey_of_false hka] at h
-  · simp [containsKey_eraseKey_of_beq hl hka] at h
+  · rwa [containsKey_removeKey_of_false hka] at h
+  · simp [containsKey_removeKey_of_beq hl hka] at h
 
-theorem findEntry?_of_perm [BEq α] [PartialEquivBEq α] {l l' : List (Σ a, β a)} {k : α} (hl : l.DistinctKeys)
-    (h : l ~ l') : l.findEntry? k = l'.findEntry? k := by
+theorem getEntry?_of_perm [BEq α] [PartialEquivBEq α] {l l' : List (Σ a, β a)} {k : α} (hl : l.DistinctKeys)
+    (h : l ~ l') : l.getEntry? k = l'.getEntry? k := by
   induction h
   · simp
   · next p t₁ t₂ _ ih₂ =>
     rcases p with ⟨k', v'⟩
-    simp only [findEntry?_cons, ih₂ hl.tail]
+    simp only [getEntry?_cons, ih₂ hl.tail]
   · next p p' t =>
     rcases p with ⟨k₁, v₁⟩
     rcases p' with ⟨k₂, v₂⟩
-    simp only [findEntry?_cons]
+    simp only [getEntry?_cons]
     cases h₂ : k₂ == k <;> cases h₁ : k₁ == k <;> try simp; done
     simp only [distinctKeys_cons_iff, containsKey_cons, Bool.or_eq_false_iff] at hl
     exact ((Bool.eq_false_iff.1 hl.2.1).elim (BEq.trans h₁ (BEq.symm h₂))).elim
@@ -1014,118 +1014,118 @@ theorem findEntry?_of_perm [BEq α] [PartialEquivBEq α] {l l' : List (Σ a, β 
 
 theorem containsKey_of_perm [BEq α] [PartialEquivBEq α] {l l' : List (Σ a, β a)} {k : α} (hl : l.DistinctKeys)
     (h : l ~ l') : l.containsKey k = l'.containsKey k := by
-  simp only [containsKey_eq_isSome_findEntry?, findEntry?_of_perm hl h]
+  simp only [containsKey_eq_isSome_getEntry?, getEntry?_of_perm hl h]
 
-theorem findValueCast?_of_perm [BEq α] [LawfulBEq α] {l l' : List (Σ a, β a)} {k : α} (hl : l.DistinctKeys)
-    (h : l ~ l') : l.findValueCast? k = l'.findValueCast? k := by
-  rw [findValueCast?_eq_findEntry?, findValueCast?_eq_findEntry?, Option.dmap_congr (findEntry?_of_perm hl h)]
+theorem getValueCast?_of_perm [BEq α] [LawfulBEq α] {l l' : List (Σ a, β a)} {k : α} (hl : l.DistinctKeys)
+    (h : l ~ l') : l.getValueCast? k = l'.getValueCast? k := by
+  rw [getValueCast?_eq_getEntry?, getValueCast?_eq_getEntry?, Option.dmap_congr (getEntry?_of_perm hl h)]
 
 section
 
 variable {β : Type v}
 
-theorem findValue?_of_perm [BEq α] [PartialEquivBEq α] {l l' : List ((_ : α) × β)} {k : α} (hl : l.DistinctKeys)
-    (h : l ~ l') : l.findValue? k = l'.findValue? k := by
-  simp only [findValue?_eq_findEntry?, findEntry?_of_perm hl h]
+theorem getValue?_of_perm [BEq α] [PartialEquivBEq α] {l l' : List ((_ : α) × β)} {k : α} (hl : l.DistinctKeys)
+    (h : l ~ l') : l.getValue? k = l'.getValue? k := by
+  simp only [getValue?_eq_getEntry?, getEntry?_of_perm hl h]
 
 theorem mem_values_of_perm [BEq α] [EquivBEq α] {l l' : List ((_ : α) × β)} {v : β} (hl : l.DistinctKeys)
     (h : l ~ l') : v ∈ l.values ↔ v ∈ l'.values := by
-  rw [mem_values_iff_exists_findValue?_eq_some hl, mem_values_iff_exists_findValue?_eq_some (hl.perm h.symm)]
-  simp only [findValue?_of_perm hl h]
+  rw [mem_values_iff_exists_getValue?_eq_some hl, mem_values_iff_exists_getValue?_eq_some (hl.perm h.symm)]
+  simp only [getValue?_of_perm hl h]
 
 end
 
-theorem perm_cons_findEntry [BEq α] {l : List (Σ a, β a)} {k : α} (h : l.containsKey k) :
-    ∃ l', l ~ l.findEntry k h :: l' := by
+theorem perm_cons_getEntry [BEq α] {l : List (Σ a, β a)} {k : α} (h : l.containsKey k) :
+    ∃ l', l ~ l.getEntry k h :: l' := by
   induction l using assoc_induction
   · simp at h
   · next k' v' t ih =>
     simp only [containsKey_cons, Bool.or_eq_true] at h
     cases hk : k' == k
     · obtain ⟨l', hl'⟩ := ih (h.resolve_left (Bool.not_eq_true _ ▸ hk))
-      rw [findEntry_cons_of_false hk]
+      rw [getEntry_cons_of_false hk]
       exact ⟨⟨k', v'⟩ :: l', (hl'.cons _).trans (Perm.swap _ _ _)⟩
-    · exact ⟨t, by rw [findEntry_cons_of_beq hk]⟩
+    · exact ⟨t, by rw [getEntry_cons_of_beq hk]⟩
 
 -- Note: this theorem becomes false if you don't assume that BEq is reflexive on α.
-theorem findEntry?_ext [BEq α] [EquivBEq α] {l l' : List (Σ a, β a)} (hl : l.DistinctKeys) (hl' : l'.DistinctKeys)
-    (h : ∀ k, l.findEntry? k = l'.findEntry? k) : l ~ l' := by
+theorem getEntry?_ext [BEq α] [EquivBEq α] {l l' : List (Σ a, β a)} (hl : l.DistinctKeys) (hl' : l'.DistinctKeys)
+    (h : ∀ k, l.getEntry? k = l'.getEntry? k) : l ~ l' := by
   induction l using assoc_induction generalizing l'
   · induction l' using assoc_induction
     · rfl
     · next k _ _ _ => simpa using h k
   · next k v t ih =>
-    have hl'k₁ : l'.findEntry? k = some ⟨k, v⟩ := by rw [← h, findEntry?_cons_self]
+    have hl'k₁ : l'.getEntry? k = some ⟨k, v⟩ := by rw [← h, getEntry?_cons_self]
     have hl'k₂ : l'.containsKey k := by
-      rw [containsKey_eq_isSome_findEntry?, hl'k₁, Option.isSome_some]
-    obtain ⟨l'', hl''⟩ := perm_cons_findEntry hl'k₂
-    rw [findEntry_eq_of_findEntry?_eq_some hl'k₁] at hl''
+      rw [containsKey_eq_isSome_getEntry?, hl'k₁, Option.isSome_some]
+    obtain ⟨l'', hl''⟩ := perm_cons_getEntry hl'k₂
+    rw [getEntry_eq_of_getEntry?_eq_some hl'k₁] at hl''
     suffices t ~ l'' from (this.cons _).trans hl''.symm
     apply ih hl.tail (hl'.perm hl''.symm).tail
     intro k'
     cases hk' : k' == k
-    · simpa only [findEntry?_of_perm hl' hl'', findEntry?_cons_of_false (BEq.symm_false hk')] using h k'
-    · simp only [findEntry?_eq_of_beq hk']
-      rw [findEntry?_eq_none.2 hl.containsKey_eq_false,
-          findEntry?_eq_none.2 (hl'.perm hl''.symm).containsKey_eq_false]
+    · simpa only [getEntry?_of_perm hl' hl'', getEntry?_cons_of_false (BEq.symm_false hk')] using h k'
+    · simp only [getEntry?_eq_of_beq hk']
+      rw [getEntry?_eq_none.2 hl.containsKey_eq_false,
+          getEntry?_eq_none.2 (hl'.perm hl''.symm).containsKey_eq_false]
 
 theorem replaceEntry_of_perm [BEq α] [EquivBEq α] {l l' : List (Σ a, β a)} {k : α} {v : β k}
     (hl : l.DistinctKeys) (h : l ~ l') : l.replaceEntry k v ~ l'.replaceEntry k v := by
-  apply findEntry?_ext hl.replaceEntry (hl.perm h.symm).replaceEntry
-  simp [findEntry?_replaceEntry, findEntry?_of_perm hl h, containsKey_of_perm hl h]
+  apply getEntry?_ext hl.replaceEntry (hl.perm h.symm).replaceEntry
+  simp [getEntry?_replaceEntry, getEntry?_of_perm hl h, containsKey_of_perm hl h]
 
 theorem insertEntry_of_perm [BEq α] [EquivBEq α] {l l' : List (Σ a, β a)} {k : α} {v : β k}
     (hl : l.DistinctKeys) (h : l ~ l') : l.insertEntry k v ~ l'.insertEntry k v := by
-  apply findEntry?_ext hl.insertEntry (hl.perm h.symm).insertEntry
-  simp [findEntry?_insertEntry, findEntry?_of_perm hl h]
+  apply getEntry?_ext hl.insertEntry (hl.perm h.symm).insertEntry
+  simp [getEntry?_insertEntry, getEntry?_of_perm hl h]
 
-theorem eraseKey_of_perm [BEq α] [EquivBEq α] {l l' : List (Σ a, β a)} {k : α}
-    (hl : l.DistinctKeys) (h : l ~ l') : l.eraseKey k ~ l'.eraseKey k := by
-  apply findEntry?_ext hl.eraseKey (hl.perm h.symm).eraseKey
-  simp [findEntry?_eraseKey hl, findEntry?_eraseKey (hl.perm h.symm), findEntry?_of_perm hl h]
+theorem removeKey_of_perm [BEq α] [EquivBEq α] {l l' : List (Σ a, β a)} {k : α}
+    (hl : l.DistinctKeys) (h : l ~ l') : l.removeKey k ~ l'.removeKey k := by
+  apply getEntry?_ext hl.removeKey (hl.perm h.symm).removeKey
+  simp [getEntry?_removeKey hl, getEntry?_removeKey (hl.perm h.symm), getEntry?_of_perm hl h]
 
 @[simp]
-theorem findEntry?_append [BEq α] {l l' : List (Σ a, β a)} {k : α} :
-    (l ++ l').findEntry? k = (l.findEntry? k).or (l'.findEntry? k) := by
+theorem getEntry?_append [BEq α] {l l' : List (Σ a, β a)} {k : α} :
+    (l ++ l').getEntry? k = (l.getEntry? k).or (l'.getEntry? k) := by
   induction l using assoc_induction
   · simp
-  · next k' v' t ih => cases h : k' == k <;> simp_all [findEntry?_cons]
+  · next k' v' t ih => cases h : k' == k <;> simp_all [getEntry?_cons]
 
-theorem findEntry?_append_of_containsKey_eq_false [BEq α] {l l' : List (Σ a, β a)} {k : α}
-    (h : l'.containsKey k = false) : (l ++ l').findEntry? k = l.findEntry? k := by
-  rw [findEntry?_append, findEntry?_eq_none.2 h, Option.or_none]
+theorem getEntry?_append_of_containsKey_eq_false [BEq α] {l l' : List (Σ a, β a)} {k : α}
+    (h : l'.containsKey k = false) : (l ++ l').getEntry? k = l.getEntry? k := by
+  rw [getEntry?_append, getEntry?_eq_none.2 h, Option.or_none]
 
 @[simp]
 theorem containsKey_append [BEq α] {l l' : List (Σ a, β a)} {k : α} :
     (l ++ l').containsKey k = (l.containsKey k || l'.containsKey k) := by
-  simp [containsKey_eq_isSome_findEntry?]
+  simp [containsKey_eq_isSome_getEntry?]
 
 theorem containsKey_append_of_not_contains_right [BEq α] {l l' : List (Σ a, β a)} {k : α}
     (hl' : l'.containsKey k = false) : (l ++ l').containsKey k = l.containsKey k := by
   simp [hl']
 
 @[simp]
-theorem findValue?_append {β : Type v} [BEq α] {l l' : List ((_ : α) × β)} {k : α} :
-    (l ++ l').findValue? k = (l.findValue? k).or (l'.findValue? k) := by
-  simp [findValue?_eq_findEntry?, Option.map_or]
+theorem getValue?_append {β : Type v} [BEq α] {l l' : List ((_ : α) × β)} {k : α} :
+    (l ++ l').getValue? k = (l.getValue? k).or (l'.getValue? k) := by
+  simp [getValue?_eq_getEntry?, Option.map_or]
 
-theorem findValue?_append_of_containsKey_eq_false {β : Type v} [BEq α] {l l' : List ((_ : α) × β)} {k : α}
-    (h : l'.containsKey k = false) : (l ++ l').findValue? k = l.findValue? k := by
-  rw [findValue?_append, findValue?_eq_none.2 h, Option.or_none]
+theorem getValue?_append_of_containsKey_eq_false {β : Type v} [BEq α] {l l' : List ((_ : α) × β)} {k : α}
+    (h : l'.containsKey k = false) : (l ++ l').getValue? k = l.getValue? k := by
+  rw [getValue?_append, getValue?_eq_none.2 h, Option.or_none]
 
-theorem findValueCast?_append_of_containsKey_eq_false [BEq α] [LawfulBEq α] {l l' : List (Σ a, β a)} {k : α}
-    (hl' : l'.containsKey k = false) : (l ++ l').findValueCast? k = l.findValueCast? k := by
-  rw [findValueCast?_eq_findEntry?, findValueCast?_eq_findEntry?, Option.dmap_congr findEntry?_append,
-    Option.dmap_congr (by rw [findEntry?_eq_none.2 hl']), Option.dmap_congr (by rw [Option.or_none])]
+theorem getValueCast?_append_of_containsKey_eq_false [BEq α] [LawfulBEq α] {l l' : List (Σ a, β a)} {k : α}
+    (hl' : l'.containsKey k = false) : (l ++ l').getValueCast? k = l.getValueCast? k := by
+  rw [getValueCast?_eq_getEntry?, getValueCast?_eq_getEntry?, Option.dmap_congr getEntry?_append,
+    Option.dmap_congr (by rw [getEntry?_eq_none.2 hl']), Option.dmap_congr (by rw [Option.or_none])]
 
 @[simp]
-theorem findKey?_append [BEq α] {l l' : List (Σ a, β a)} {k : α} :
-    (l ++ l').findKey? k = (l.findKey? k).or (l'.findKey? k) := by
-  simp [findKey?_eq_findEntry?, Option.map_or]
+theorem getKey?_append [BEq α] {l l' : List (Σ a, β a)} {k : α} :
+    (l ++ l').getKey? k = (l.getKey? k).or (l'.getKey? k) := by
+  simp [getKey?_eq_getEntry?, Option.map_or]
 
-theorem findKey?_append_of_containsKey_eq_false [BEq α] {l l' : List (Σ a, β a)} {k : α}
-    (h : l'.containsKey k = false) : (l ++ l').findKey? k = l.findKey? k := by
-  rw [findKey?_append, findKey?_eq_none.2 h, Option.or_none]
+theorem getKey?_append_of_containsKey_eq_false [BEq α] {l l' : List (Σ a, β a)} {k : α}
+    (h : l'.containsKey k = false) : (l ++ l').getKey? k = l.getKey? k := by
+  rw [getKey?_append, getKey?_eq_none.2 h, Option.or_none]
 
 theorem replaceEntry_append_of_containsKey_left [BEq α] {l l' : List (Σ a, β a)} {k : α}
     {v : β k} (h : l.containsKey k) : (l ++ l').replaceEntry k v = l.replaceEntry k v ++ l' := by
@@ -1159,12 +1159,12 @@ theorem insertEntry_append_of_not_contains_right [BEq α] {l l' : List (Σ a, β
   · simp [insertEntry, containsKey_append, h, h']
   · simp [insertEntry, containsKey_append, h, h', replaceEntry_append_of_containsKey_left h]
 
-theorem eraseKey_append_of_containsKey_right_eq_false [BEq α] {l l' : List (Σ a, β a)} {k : α}
-    (h : l'.containsKey k = false) : (l ++ l').eraseKey k = l.eraseKey k ++ l' := by
+theorem removeKey_append_of_containsKey_right_eq_false [BEq α] {l l' : List (Σ a, β a)} {k : α}
+    (h : l'.containsKey k = false) : (l ++ l').removeKey k = l.removeKey k ++ l' := by
   induction l using assoc_induction
-  · simp [eraseKey_of_containsKey_eq_false h]
+  · simp [removeKey_of_containsKey_eq_false h]
   · next k' v' t ih =>
-    rw [cons_append, eraseKey_cons, eraseKey_cons]
+    rw [cons_append, removeKey_cons, removeKey_cons]
     cases k' == k
     · rw [cond_false, cond_false, ih, cons_append]
     · rw [cond_true, cond_true]
