Hashmap/DHashMap/Internal/RawLemmas.lean
@@ -42,48 +42,48 @@ namespace Raw₀
 variable (m : Raw₀ α β) (h : m.1.WF)
 
 @[simp]
-theorem findEntry?_empty {a : α} {c : Nat} : (empty c : Raw₀ α β).findEntry? a = none := by
-  simp [findEntry?]
+theorem getEntry?_empty {a : α} {c : Nat} : (empty c : Raw₀ α β).getEntry? a = none := by
+  simp [getEntry?]
 
 @[simp]
-theorem findConst?_empty {β : Type v} {a : α} {c : Nat} : (empty c : Raw₀ α (fun _ => β)).findConst? a = none := by
-  simp [findConst?]
+theorem Const.get?_empty {β : Type v} {a : α} {c : Nat} : Const.get? (empty c : Raw₀ α (fun _ => β)) a = none := by
+  simp [Const.get?]
 
-theorem findEntry?_insertB (a k : α) (b : β a) :
-    (m.insertB a b).1.findEntry? k = bif a == k then some ⟨a, b⟩ else m.findEntry? k := by
-  rw [findEntry?_eq_findEntry? h.out.insertB, findEntry?_eq_findEntry? h.out,
-    List.findEntry?_of_perm h.out.insertB.distinct (toListModel_insertB h.out),
-    List.findEntry?_insertEntry]
+theorem getEntry?_containsThenInsert (a k : α) (b : β a) :
+    (m.containsThenInsert a b).1.getEntry? k = bif a == k then some ⟨a, b⟩ else m.getEntry? k := by
+  rw [getEntry?_eq_getEntry? h.out.containsThenInsert, getEntry?_eq_getEntry? h.out,
+    List.getEntry?_of_perm h.out.containsThenInsert.distinct (toListModel_containsThenInsert h.out),
+    List.getEntry?_insertEntry]
 
-theorem findEntry?_insert (a k : α) (b : β a) :
-    (m.insert a b).findEntry? k = bif a == k then some ⟨a, b⟩ else m.findEntry? k := by
-  rw [findEntry?_eq_findEntry? h.out.insert, findEntry?_eq_findEntry? h.out,
-    List.findEntry?_of_perm h.out.insert.distinct (toListModel_insert h.out),
-    List.findEntry?_insertEntry]
+theorem getEntry?_insert (a k : α) (b : β a) :
+    (m.insert a b).getEntry? k = bif a == k then some ⟨a, b⟩ else m.getEntry? k := by
+  rw [getEntry?_eq_getEntry? h.out.insert, getEntry?_eq_getEntry? h.out,
+    List.getEntry?_of_perm h.out.insert.distinct (toListModel_insert h.out),
+    List.getEntry?_insertEntry]
 
-theorem findConst?_insertB {β : Type v} (m : Raw₀ α (fun _ => β)) (h : m.1.WF) (a k : α) (b : β) :
-    (m.insertB a b).1.findConst? k = bif a == k then some b else m.findConst? k := by
-  rw [findConst?_eq_findValue? h.out.insertB, findConst?_eq_findValue? h.out,
-    List.findValue?_of_perm h.out.insertB.distinct (toListModel_insertB h.out),
-    List.findValue?_insertEntry]
+theorem Const.get?_containsThenInsert {β : Type v} (m : Raw₀ α (fun _ => β)) (h : m.1.WF) (a k : α) (b : β) :
+    Const.get? (m.containsThenInsert a b).1 k = bif a == k then some b else Const.get? m k := by
+  rw [Const.get?_eq_getValue? h.out.containsThenInsert, Const.get?_eq_getValue? h.out,
+    List.getValue?_of_perm h.out.containsThenInsert.distinct (toListModel_containsThenInsert h.out),
+    List.getValue?_insertEntry]
 
-theorem findConst?_insert {β : Type v} (m : Raw₀ α (fun _ => β)) (h : m.1.WF) (a k : α) (b : β) :
-    (m.insert a b).findConst? k = bif a == k then some b else m.findConst? k := by
-  rw [findConst?_eq_findValue? h.out.insert, findConst?_eq_findValue? h.out,
-    List.findValue?_of_perm h.out.insert.distinct (toListModel_insert h.out),
-    List.findValue?_insertEntry]
+theorem Const.get?_insert {β : Type v} (m : Raw₀ α (fun _ => β)) (h : m.1.WF) (a k : α) (b : β) :
+    Const.get? (m.insert a b) k = bif a == k then some b else Const.get? m k := by
+  rw [Const.get?_eq_getValue? h.out.insert, Const.get?_eq_getValue? h.out,
+    List.getValue?_of_perm h.out.insert.distinct (toListModel_insert h.out),
+    List.getValue?_insertEntry]
 
-theorem findConst?_congr {β : Type v} (m : Raw₀ α (fun _ => β)) (h : m.1.WF) {a b : α} (hab : a == b) :
-    m.findConst? a = m.findConst? b := by
-  rw [findConst?_eq_findValue? h.out, findConst?_eq_findValue? h.out, List.findValue?_eq_of_beq hab]
+theorem Const.get?_congr {β : Type v} (m : Raw₀ α (fun _ => β)) (h : m.1.WF) {a b : α} (hab : a == b) :
+    Const.get? m a = Const.get? m b := by
+  rw [Const.get?_eq_getValue? h.out, Const.get?_eq_getValue? h.out, List.getValue?_eq_of_beq hab]
 
 @[simp]
 theorem contains_empty {a : α} {c : Nat} : (empty c : Raw₀ α β).contains a = false := by
   simp [contains]
 
-theorem contains_insertB (a k : α) (b : β a) : (m.insertB a b).1.contains k = ((a == k) || m.contains k) := by
-  rw [contains_eq_containsKey h.out.insertB, contains_eq_containsKey h.out,
-    List.containsKey_of_perm h.out.insertB.distinct (toListModel_insertB h.out),
+theorem contains_containsThenInsert (a k : α) (b : β a) : (m.containsThenInsert a b).1.contains k = ((a == k) || m.contains k) := by
+  rw [contains_eq_containsKey h.out.containsThenInsert, contains_eq_containsKey h.out,
+    List.containsKey_of_perm h.out.containsThenInsert.distinct (toListModel_containsThenInsert h.out),
     List.containsKey_insertEntry]
 
 theorem contains_insert (a k : α) (b : β a) : (m.insert a b).contains k = ((a == k) || m.contains k) := by
@@ -91,51 +91,51 @@ theorem contains_insert (a k : α) (b : β a) : (m.insert a b).contains k = ((a 
     List.containsKey_of_perm h.out.insert.distinct (toListModel_insert h.out),
     List.containsKey_insertEntry]
 
-theorem contains_eq_isSome_findEntry? {a : α} : m.contains a = (m.findEntry? a).isSome := by
-  rw [findEntry?_eq_findEntry? h.out, contains_eq_containsKey h.out, List.containsKey_eq_isSome_findEntry?]
+theorem contains_eq_isSome_getEntry? {a : α} : m.contains a = (m.getEntry? a).isSome := by
+  rw [getEntry?_eq_getEntry? h.out, contains_eq_containsKey h.out, List.containsKey_eq_isSome_getEntry?]
 
-theorem findEntry?_eq_some (a : α) (p : Σ a, β a) (h : m.findEntry? a = some p) : p.1 == a :=
-  AssocList.findEntry?_eq_some h
+theorem getEntry?_eq_some (a : α) (p : Σ a, β a) (h : m.getEntry? a = some p) : p.1 == a :=
+  AssocList.getEntry?_eq_some h
 
-theorem mem_values_iff_exists_findConst?_eq_some {β : Type v} (m : Raw₀ α (fun _ => β)) (h : m.1.WF) {v : β} :
-    v ∈ m.1.values ↔ ∃ k, m.findConst? k = some v := by
-  rw [mem_values_iff_mem_values_toListModel, List.mem_values_iff_exists_findValue?_eq_some h.out.distinct]
-  simp only [findConst?_eq_findValue? h.out]
+theorem Const.mem_values_iff_exists_get?_eq_some {β : Type v} (m : Raw₀ α (fun _ => β)) (h : m.1.WF) {v : β} :
+    v ∈ m.1.values ↔ ∃ k, Const.get? m k = some v := by
+  rw [mem_values_iff_mem_values_toListModel, List.mem_values_iff_exists_getValue?_eq_some h.out.distinct]
+  simp only [Const.get?_eq_getValue? h.out]
 
 @[simp]
 theorem values_empty {β : Type v} {c} : (empty c : Raw₀ α (fun _ => β)).1.values = [] := by
   simpa using Raw.values_perm_values_toListModel (m := (empty c : Raw₀ α (fun _ => β)).1)
 
-theorem mem_values_insertB {β : Type v} (m : Raw₀ α (fun _ => β)) (h : m.1.WF) {a : α} {b v : β} :
-    v ∈ (m.insertB a b).1.1.values ↔ b = v ∨ ∃ k, (a == k) = false ∧ m.findConst? k = some v := by
-  rw [mem_values_iff_mem_values_toListModel, List.mem_values_of_perm h.out.insertB.distinct (toListModel_insertB h.out),
+theorem mem_values_containsThenInsert {β : Type v} (m : Raw₀ α (fun _ => β)) (h : m.1.WF) {a : α} {b v : β} :
+    v ∈ (m.containsThenInsert a b).1.1.values ↔ b = v ∨ ∃ k, (a == k) = false ∧ Const.get? m k = some v := by
+  rw [mem_values_iff_mem_values_toListModel, List.mem_values_of_perm h.out.containsThenInsert.distinct (toListModel_containsThenInsert h.out),
     List.mem_values_insertEntry h.out.distinct]
-  simp only [findConst?_eq_findValue? h.out]
+  simp only [Const.get?_eq_getValue? h.out]
 
 theorem mem_values_insert {β : Type v} (m : Raw₀ α (fun _ => β)) (h : m.1.WF) {a : α} {b v : β} :
-    v ∈ (m.insert a b).1.values ↔ b = v ∨ ∃ k, (a == k) = false ∧ m.findConst? k = some v := by
+    v ∈ (m.insert a b).1.values ↔ b = v ∨ ∃ k, (a == k) = false ∧ Const.get? m k = some v := by
   rw [mem_values_iff_mem_values_toListModel, List.mem_values_of_perm h.out.insert.distinct (toListModel_insert h.out),
     List.mem_values_insertEntry h.out.distinct]
-  simp only [findConst?_eq_findValue? h.out]
+  simp only [Const.get?_eq_getValue? h.out]
 
 @[simp]
 theorem isEmpty_empty {c} : (empty c : Raw₀ α β).1.isEmpty := by
   rw [Raw.isEmpty_eq_isEmpty wfImp_empty, toListModel_buckets_empty, List.isEmpty_nil]
 
 @[simp]
-theorem isEmpty_insertB {a : α} {b : β a} : (m.insertB a b).1.1.isEmpty = false := by
-  rw [Raw.isEmpty_eq_isEmpty h.out.insertB, (toListModel_insertB h.out).isEmpty_eq, List.isEmpty_insertEntry]
+theorem isEmpty_containsThenInsert {a : α} {b : β a} : (m.containsThenInsert a b).1.1.isEmpty = false := by
+  rw [Raw.isEmpty_eq_isEmpty h.out.containsThenInsert, (toListModel_containsThenInsert h.out).isEmpty_eq, List.isEmpty_insertEntry]
 
 @[simp]
 theorem isEmpty_insert {a : α} {b : β a} : (m.insert a b).1.isEmpty = false := by
   rw [Raw.isEmpty_eq_isEmpty h.out.insert, (toListModel_insert h.out).isEmpty_eq, List.isEmpty_insertEntry]
 
-theorem findEntry?_of_isEmpty {a : α} (h' : m.1.isEmpty = true) : m.findEntry? a = none := by
-  simp_all [findEntry?_eq_findEntry? h.out, Raw.isEmpty_eq_isEmpty h.out, List.isEmpty_iff]
+theorem getEntry?_of_isEmpty {a : α} (h' : m.1.isEmpty = true) : m.getEntry? a = none := by
+  simp_all [getEntry?_eq_getEntry? h.out, Raw.isEmpty_eq_isEmpty h.out, List.isEmpty_iff]
 
-theorem findConst?_of_isEmpty {a : α} {β : Type v} (m : Raw₀ α (fun _ => β)) (h : m.1.WF) (h' : m.1.isEmpty = true) :
-    m.findConst? a = none := by
-  simp_all [findConst?_eq_findValue? h.out, Raw.isEmpty_eq_isEmpty h.out, List.isEmpty_iff]
+theorem Const.get?_of_isEmpty {a : α} {β : Type v} (m : Raw₀ α (fun _ => β)) (h : m.1.WF) (h' : m.1.isEmpty = true) :
+    Const.get? m a = none := by
+  simp_all [Const.get?_eq_getValue? h.out, Raw.isEmpty_eq_isEmpty h.out, List.isEmpty_iff]
 
 theorem contains_of_isEmpty {a : α} (h' : m.1.isEmpty = true) : m.contains a = false := by
   simp_all [contains_eq_containsKey h.out, Raw.isEmpty_eq_isEmpty h.out, List.isEmpty_iff]
