Hashmap/DHashMap/Lemmas.lean
@@ -18,32 +18,32 @@ namespace Raw
 variable (m : Raw α β) (h : m.WF)
 
 @[simp]
-theorem findEntry?_empty {a : α} {c : Nat} : (empty c : Raw α β).findEntry? a = none := by
-  rw [empty_eq, findEntry?_eq WF.empty₀, Raw₀.findEntry?_empty]
+theorem getEntry?_empty {a : α} {c : Nat} : (empty c : Raw α β).getEntry? a = none := by
+  rw [empty_eq, getEntry?_eq WF.empty₀, Raw₀.getEntry?_empty]
 
 @[simp]
-theorem findEntry?_emptyc {a : α} : (∅ : Raw α β).findEntry? a = none :=
-  findEntry?_empty
+theorem getEntry?_emptyc {a : α} : (∅ : Raw α β).getEntry? a = none :=
+  getEntry?_empty
 
 @[simp]
-theorem findConst?_empty {β : Type v} {a : α} {c : Nat} : (empty c : Raw α (fun _ => β)).findConst? a = none := by
-  rw [empty_eq, findConst?_eq WF.empty₀, Raw₀.findConst?_empty]
+theorem Const.get?_empty {β : Type v} {a : α} {c : Nat} : Const.get? (empty c : Raw α (fun _ => β)) a = none := by
+  rw [empty_eq, Const.get?_eq WF.empty₀, Raw₀.Const.get?_empty]
 
 @[simp]
-theorem findConst?_emptyc {β : Type v} {a : α} : (∅ : Raw α (fun _ => β)).findConst? a = none :=
-  findConst?_empty
+theorem getConst?_emptyc {β : Type v} {a : α} : Const.get? (∅ : Raw α (fun _ => β)) a = none :=
+  Const.get?_empty
 
-theorem findEntry?_insert {a k : α} {b : β a} :
-    (m.insert a b).findEntry? k = bif a == k then some ⟨a, b⟩ else m.findEntry? k := by
-  rw [insert_eq h, findEntry?_eq h, findEntry?_eq h.insert₀, Raw₀.findEntry?_insert ⟨m, _⟩ h]
+theorem getEntry?_insert {a k : α} {b : β a} :
+    (m.insert a b).getEntry? k = bif a == k then some ⟨a, b⟩ else m.getEntry? k := by
+  rw [insert_eq h, getEntry?_eq h, getEntry?_eq h.insert₀, Raw₀.getEntry?_insert ⟨m, _⟩ h]
 
-theorem findConst?_insert {β : Type v} (m : Raw α (fun _ => β)) (h : m.WF) (a k : α) (b : β) :
-    (m.insert a b).findConst? k = bif a == k then some b else m.findConst? k := by
-  rw [insert_eq h, findConst?_eq h, findConst?_eq h.insert₀, Raw₀.findConst?_insert ⟨m, _⟩ h]
+theorem Const.get?_insert {β : Type v} (m : Raw α (fun _ => β)) (h : m.WF) (a k : α) (b : β) :
+    Const.get? (m.insert a b) k = bif a == k then some b else Const.get? m k := by
+  rw [insert_eq h, Const.get?_eq h, Const.get?_eq h.insert₀, Raw₀.Const.get?_insert ⟨m, _⟩ h]
 
-theorem findConst?_congr {β : Type v} (m : Raw α (fun _ => β)) (h : m.WF) {a b : α} (hab : a == b) :
-    m.findConst? a = m.findConst? b := by
-  rw [findConst?_eq h, findConst?_eq h, Raw₀.findConst?_congr ⟨m, _⟩ h hab]
+theorem Const.get?_congr {β : Type v} (m : Raw α (fun _ => β)) (h : m.WF) {a b : α} (hab : a == b) :
+    Const.get? m a = Const.get? m b := by
+  rw [Const.get?_eq h, Const.get?_eq h, Raw₀.Const.get?_congr ⟨m, _⟩ h hab]
 
 @[simp]
 theorem contains_empty {a : α} {c : Nat} : (empty c : Raw α β).contains a = false := by
@@ -56,13 +56,13 @@ theorem contains_emptyc {a : α} : (∅ : Raw α β).contains a = false :=
 theorem contains_insert {a k : α} {b : β a} : (m.insert a b).contains k = ((a == k) || m.contains k) := by
   rw [insert_eq h, contains_eq h, contains_eq h.insert₀, Raw₀.contains_insert ⟨m, _⟩ h]
 
-theorem contains_eq_isSome_findEntry? {a : α} : m.contains a = (m.findEntry? a).isSome := by
-  rw [contains_eq h, findEntry?_eq h, Raw₀.contains_eq_isSome_findEntry? ⟨m, _⟩ h]
+theorem contains_eq_isSome_getEntry? {a : α} : m.contains a = (m.getEntry? a).isSome := by
+  rw [contains_eq h, getEntry?_eq h, Raw₀.contains_eq_isSome_getEntry? ⟨m, _⟩ h]
 
-theorem mem_values_iff_exists_findConst?_eq_some {β : Type v} (m : Raw α (fun _ => β)) (h : m.WF) {v : β} :
-    v ∈ m.values ↔ ∃ k, m.findConst? k = some v := by
-  rw [Raw₀.mem_values_iff_exists_findConst?_eq_some ⟨m, h.size_buckets_pos⟩ h]
-  simp only [findConst?_eq h]
+theorem Const.mem_values_iff_exists_get?_eq_some {β : Type v} (m : Raw α (fun _ => β)) (h : m.WF) {v : β} :
+    v ∈ m.values ↔ ∃ k, Const.get? m k = some v := by
+  rw [Raw₀.Const.mem_values_iff_exists_get?_eq_some ⟨m, h.size_buckets_pos⟩ h]
+  simp only [Const.get?_eq h]
 
 @[simp]
 theorem values_empty {β : Type v} {c} : (empty c : Raw α (fun _ => β)).values = [] :=
@@ -73,9 +73,9 @@ theorem values_emptyc {β : Type v} : (∅ : Raw α (fun _ => β)).values = [] :
   values_empty
 
 theorem mem_values_insert {β : Type v} {m : Raw α (fun _ => β)} (h : m.WF) {a : α} {b v : β} :
-    v ∈ (m.insert a b).values ↔ b = v ∨ ∃ k, (a == k) = false ∧ m.findConst? k = some v := by
+    v ∈ (m.insert a b).values ↔ b = v ∨ ∃ k, (a == k) = false ∧ Const.get? m k = some v := by
   rw [insert_eq h, Raw₀.mem_values_insert ⟨m, h.size_buckets_pos⟩ h]
-  simp only [findConst?_eq h]
+  simp only [Const.get?_eq h]
 
 @[simp]
 theorem isEmpty_empty {c} : (empty c : Raw α β).isEmpty :=
@@ -86,19 +86,19 @@ theorem isEmpty_emptyc : (∅ : Raw α β).isEmpty :=
   isEmpty_empty
 
 @[simp]
-theorem isEmpty_insertB {a : α} {b : β a} : (m.insertB a b).1.isEmpty = false := by
-  rw [insertB_eq h, Raw₀.isEmpty_insertB ⟨m, _⟩ h]
+theorem isEmpty_containsThenInsert {a : α} {b : β a} : (m.containsThenInsert a b).1.isEmpty = false := by
+  rw [containsThenInsert_eq h, Raw₀.isEmpty_containsThenInsert ⟨m, _⟩ h]
 
 @[simp]
 theorem isEmpty_insert {a : α} {b : β a} : (m.insert a b).isEmpty = false := by
   rw [insert_eq h, Raw₀.isEmpty_insert ⟨m, _⟩ h]
 
-theorem findEntry?_of_isEmpty {a : α} (h' : m.isEmpty = true) : m.findEntry? a = none := by
-  rw [findEntry?_eq h, Raw₀.findEntry?_of_isEmpty ⟨m, _⟩ h h']
+theorem getEntry?_of_isEmpty {a : α} (h' : m.isEmpty = true) : m.getEntry? a = none := by
+  rw [getEntry?_eq h, Raw₀.getEntry?_of_isEmpty ⟨m, _⟩ h h']
 
-theorem findConst?_of_isEmpty {a : α} {β : Type v} {m : Raw α (fun _ => β)} (h : m.WF) (h' : m.isEmpty = true) :
-    m.findConst? a = none := by
-  rw [findConst?_eq h, Raw₀.findConst?_of_isEmpty ⟨m, _⟩ h h']
+theorem Const.get?_of_isEmpty {a : α} {β : Type v} {m : Raw α (fun _ => β)} (h : m.WF) (h' : m.isEmpty = true) :
+    Const.get? m a = none := by
+  rw [Const.get?_eq h, Raw₀.Const.get?_of_isEmpty ⟨m, _⟩ h h']
 
 theorem contains_of_isEmpty {a : α} (h' : m.isEmpty = true) : m.contains a = false := by
   rw [contains_eq h, Raw₀.contains_of_isEmpty ⟨m, _⟩ h h']
@@ -113,32 +113,32 @@ section
 variable (m : DHashMap α β)
 
 @[simp]
-theorem findEntry?_empty {a : α} {c : Nat} : (empty c : DHashMap α β).findEntry? a = none :=
-  Raw₀.findEntry?_empty
+theorem getEntry?_empty {a : α} {c : Nat} : (empty c : DHashMap α β).getEntry? a = none :=
+  Raw₀.getEntry?_empty
 
 @[simp]
-theorem findEntry?_emptyc {a : α} : (∅ : DHashMap α β).findEntry? a = none :=
-  Raw₀.findEntry?_empty
+theorem getEntry?_emptyc {a : α} : (∅ : DHashMap α β).getEntry? a = none :=
+  Raw₀.getEntry?_empty
 
 @[simp]
-theorem findConst?_empty {β : Type v} {a : α} {c : Nat} : (empty c : DHashMap α (fun _ => β)).findConst? a = none :=
-  Raw₀.findConst?_empty
+theorem Const.get?_empty {β : Type v} {a : α} {c : Nat} : Const.get? (empty c : DHashMap α (fun _ => β)) a = none :=
+  Raw₀.Const.get?_empty
 
 @[simp]
-theorem findConst?_emptyc {β : Type v} {a : α} : (∅ : DHashMap α (fun _ => β)).findConst? a = none :=
-  Raw₀.findConst?_empty
+theorem Const.get?_emptyc {β : Type v} {a : α} : Const.get? (∅ : DHashMap α (fun _ => β)) a = none :=
+  Raw₀.Const.get?_empty
 
-theorem findEntry?_insert (a k : α) (b : β a) :
-    (m.insert a b).findEntry? k = bif a == k then some ⟨a, b⟩ else m.findEntry? k :=
-  Raw₀.findEntry?_insert ⟨m.1, _⟩ m.2 a k b
+theorem getEntry?_insert (a k : α) (b : β a) :
+    (m.insert a b).getEntry? k = bif a == k then some ⟨a, b⟩ else m.getEntry? k :=
+  Raw₀.getEntry?_insert ⟨m.1, _⟩ m.2 a k b
 
-theorem findConst?_insert {β : Type v} (m : DHashMap α (fun _ => β)) (a k : α) (b : β) :
-    (m.insert a b).findConst? k = bif a == k then some b else m.findConst? k :=
-  Raw₀.findConst?_insert ⟨m.1, _⟩ m.2 _ _ _
+theorem Const.get?_insert {β : Type v} (m : DHashMap α (fun _ => β)) (a k : α) (b : β) :
+    Const.get? (m.insert a b) k = bif a == k then some b else Const.get? m k :=
+  Raw₀.Const.get?_insert ⟨m.1, _⟩ m.2 ..
 
-theorem findConst?_congr {β : Type v} (m : DHashMap α (fun _ => β)) {a b : α} (hab : a == b) :
-    m.findConst? a = m.findConst? b :=
-  Raw₀.findConst?_congr ⟨m.1, _⟩ m.2 hab
+theorem Const.get?_congr {β : Type v} (m : DHashMap α (fun _ => β)) {a b : α} (hab : a == b) :
+    Const.get? m a = Const.get? m b :=
+  Raw₀.Const.get?_congr ⟨m.1, _⟩ m.2 hab
 
 @[simp]
 theorem contains_empty {a : α} {c : Nat} : (empty c : DHashMap α β).contains a = false :=
@@ -151,15 +151,15 @@ theorem contains_emptyc {a : α} : (∅ : DHashMap α β).contains a = false :=
 theorem contains_insert {a k : α} {b : β a} : (m.insert a b).contains k = ((a == k) || m.contains k) :=
   Raw₀.contains_insert ⟨m.1, _⟩ m.2 _ _ _
 
-theorem contains_eq_isSome_findEntry? {a : α} : m.contains a = (m.findEntry? a).isSome :=
-  Raw₀.contains_eq_isSome_findEntry? ⟨m.1, _⟩ m.2
+theorem contains_eq_isSome_getEntry? {a : α} : m.contains a = (m.getEntry? a).isSome :=
+  Raw₀.contains_eq_isSome_getEntry? ⟨m.1, _⟩ m.2
 
-theorem findEntry?_eq_some {a : α} {p : Σ a, β a} (h : m.findEntry? a = some p) : p.1 == a :=
-  Raw₀.findEntry?_eq_some ⟨m.1, _⟩ _ _ h
+theorem getEntry?_eq_some {a : α} {p : Σ a, β a} (h : m.getEntry? a = some p) : p.1 == a :=
+  Raw₀.getEntry?_eq_some ⟨m.1, _⟩ _ _ h
 
-theorem mem_values_iff_exists_findConst?_eq_some {β : Type v} (m : DHashMap α (fun _ => β)) {v : β} :
-    v ∈ m.values ↔ ∃ k, m.findConst? k = some v :=
-  Raw₀.mem_values_iff_exists_findConst?_eq_some ⟨m.1, _⟩ m.2
+theorem Const.mem_values_iff_exists_get?_eq_some {β : Type v} (m : DHashMap α (fun _ => β)) {v : β} :
+    v ∈ m.values ↔ ∃ k, Const.get? m k = some v :=
+  Raw₀.Const.mem_values_iff_exists_get?_eq_some ⟨m.1, _⟩ m.2
 
 @[simp]
 theorem values_empty {β : Type v} {c} : (empty c : DHashMap α (fun _ => β)).values = [] :=
@@ -170,7 +170,7 @@ theorem values_emptyc {β : Type v} : (∅ : DHashMap α (fun _ => β)).values =
   values_empty
 
 theorem mem_values_insert {β : Type v} {m : DHashMap α (fun _ => β)} {a : α} {b v : β} :
-    v ∈ (m.insert a b).values ↔ b = v ∨ ∃ k, (a == k) = false ∧ m.findConst? k = some v :=
+    v ∈ (m.insert a b).values ↔ b = v ∨ ∃ k, (a == k) = false ∧ Const.get? m k = some v :=
   Raw₀.mem_values_insert ⟨m.1, _⟩ m.2
 
 @[simp]
@@ -182,19 +182,19 @@ theorem isEmpty_emptyc : (∅ : DHashMap α β).isEmpty :=
   isEmpty_empty
 
 @[simp]
-theorem isEmpty_insertB {a : α} {b : β a} : (m.insertB a b).1.isEmpty = false :=
-  Raw₀.isEmpty_insertB ⟨m.1, _⟩ m.2
+theorem isEmpty_containsThenInsert {a : α} {b : β a} : (m.containsThenInsert a b).1.isEmpty = false :=
+  Raw₀.isEmpty_containsThenInsert ⟨m.1, _⟩ m.2
 
 @[simp]
 theorem isEmpty_insert {a : α} {b : β a} : (m.insert a b).isEmpty = false :=
   Raw₀.isEmpty_insert ⟨m.1, _⟩ m.2
 
-theorem findEntry?_of_isEmpty {a : α} (h : m.isEmpty = true) : m.findEntry? a = none :=
-  Raw₀.findEntry?_of_isEmpty ⟨m.1, _⟩ m.2 h
+theorem getEntry?_of_isEmpty {a : α} (h : m.isEmpty = true) : m.getEntry? a = none :=
+  Raw₀.getEntry?_of_isEmpty ⟨m.1, _⟩ m.2 h
 
-theorem findConst?_of_isEmpty {a : α} {β : Type v} {m : DHashMap α (fun _ => β)} (h : m.isEmpty = true) :
-    m.findConst? a = none :=
-  Raw₀.findConst?_of_isEmpty ⟨m.1, _⟩ m.2 h
+theorem Const.get?_of_isEmpty {a : α} {β : Type v} {m : DHashMap α (fun _ => β)} (h : m.isEmpty = true) :
+    Const.get? m a = none :=
+  Raw₀.Const.get?_of_isEmpty ⟨m.1, _⟩ m.2 h
 
 theorem contains_of_isEmpty {a : α} (h : m.isEmpty = true) : m.contains a = false :=
   Raw₀.contains_of_isEmpty ⟨m.1, _⟩ m.2 h
