Hashmap/HashMap/Lemmas.lean
@@ -22,31 +22,31 @@ variable (m : Raw α β) (h : m.WF)
 @[simp] theorem inner_empty {c : Nat} : (empty c : Raw α β).inner = DHashMap.Raw.empty c := rfl
 
 @[simp]
-theorem findEntry?_empty {a : α} {c : Nat} : (empty c : Raw α β).findEntry? a = none := by
-  simp [findEntry?]
+theorem getEntry?_empty {a : α} {c : Nat} : (empty c : Raw α β).getEntry? a = none := by
+  simp [getEntry?]
 
 @[simp]
-theorem findEntry?_emptyc {a : α} : (∅ : Raw α β).findEntry? a = none := by
-  simp [findEntry?]
+theorem getEntry?_emptyc {a : α} : (∅ : Raw α β).getEntry? a = none := by
+  simp [getEntry?]
 
 @[simp]
-theorem find?_empty {a : α} {c : Nat} : (empty c : Raw α β).find? a = none := by
-  simp [find?]
+theorem get?_empty {a : α} {c : Nat} : (empty c : Raw α β).get? a = none := by
+  simp [get?]
 
 @[simp]
-theorem find?_emptyc {a : α} : (∅ : Raw α β).find? a = none := by
-  simp [find?]
+theorem get?_emptyc {a : α} : (∅ : Raw α β).get? a = none := by
+  simp [get?]
 
-theorem findEntry?_insert {a k : α} {b : β} :
-    (m.insert a b).findEntry? k = bif a == k then some (a, b) else m.findEntry? k := by
-  simp [findEntry?, insert, DHashMap.Raw.findEntry?_insert _ h, apply_bif (Option.map Sigma.toProd)]
+theorem getEntry?_insert {a k : α} {b : β} :
+    (m.insert a b).getEntry? k = bif a == k then some (a, b) else m.getEntry? k := by
+  simp [getEntry?, insert, DHashMap.Raw.getEntry?_insert _ h, apply_bif (Option.map Sigma.toProd)]
 
-theorem find?_insert {a k : α} {b : β} :
-    (m.insert a b).find? k = bif a == k then some b else m.find? k := by
-  simp [find?, insert, DHashMap.Raw.findConst?_insert _ h]
+theorem get?_insert {a k : α} {b : β} :
+    (m.insert a b).get? k = bif a == k then some b else m.get? k := by
+  simp [get?, insert, DHashMap.Raw.Const.get?_insert _ h]
 
-theorem find?_congr {a b : α} (hab : a == b) : m.find? a = m.find? b := by
-  simp [find?, DHashMap.Raw.findConst?_congr _ h hab]
+theorem get?_congr {a b : α} (hab : a == b) : m.get? a = m.get? b := by
+  simp [get?, DHashMap.Raw.Const.get?_congr _ h hab]
 
 @[simp]
 theorem contains_empty {a : α} {c : Nat} : (empty c : Raw α β).contains a = false := by
@@ -59,9 +59,9 @@ theorem contains_emptyc {a : α} : (∅ : Raw α β).contains a = false := by
 theorem contains_insert {a k : α} {b : β} : (m.insert a b).contains k = ((a == k) || m.contains k) := by
   simp [contains, insert, DHashMap.Raw.contains_insert _ h]
 
-theorem mem_values_iff_exists_find?_eq_some {β : Type v} (m : Raw α β) (h : m.WF) {v : β} :
-    v ∈ m.values ↔ ∃ k, m.find? k = some v := by
-  simp [values, find?, DHashMap.Raw.mem_values_iff_exists_findConst?_eq_some _ h]
+theorem mem_values_iff_exists_get?_eq_some {β : Type v} (m : Raw α β) (h : m.WF) {v : β} :
+    v ∈ m.values ↔ ∃ k, m.get? k = some v := by
+  simp [values, get?, DHashMap.Raw.Const.mem_values_iff_exists_get?_eq_some _ h]
 
 @[simp]
 theorem values_empty {β : Type v} {c} : (empty c : Raw α β).values = [] := by
@@ -72,8 +72,8 @@ theorem values_emptyc {β : Type v} : (∅ : Raw α β).values = [] := by
   simp [values]
 
 theorem mem_values_insert {β : Type v} {m : Raw α β} (h : m.WF) {a : α} {b v : β} :
-    v ∈ (m.insert a b).values ↔ b = v ∨ ∃ k, (a == k) = false ∧ m.find? k = some v := by
-  simp [values, find?, insert, DHashMap.Raw.mem_values_insert h]
+    v ∈ (m.insert a b).values ↔ b = v ∨ ∃ k, (a == k) = false ∧ m.get? k = some v := by
+  simp [values, get?, insert, DHashMap.Raw.mem_values_insert h]
 
 end Raw
 
@@ -85,31 +85,31 @@ variable (m : HashMap α β)
 @[simp] theorem inner_empty {c : Nat} : (empty c : HashMap α β).inner = DHashMap.empty c := rfl
 
 @[simp]
-theorem findEntry?_empty {a : α} {c : Nat} : (empty c : HashMap α β).findEntry? a = none := by
-  simp [findEntry?]
+theorem getEntry?_empty {a : α} {c : Nat} : (empty c : HashMap α β).getEntry? a = none := by
+  simp [getEntry?]
 
 @[simp]
-theorem findEntry?_emptyc {a : α} : (∅ : HashMap α β).findEntry? a = none := by
-  simp [findEntry?]
+theorem getEntry?_emptyc {a : α} : (∅ : HashMap α β).getEntry? a = none := by
+  simp [getEntry?]
 
 @[simp]
-theorem find?_empty {a : α} {c : Nat} : (empty c : HashMap α β).find? a = none := by
-  simp [find?]
+theorem get?_empty {a : α} {c : Nat} : (empty c : HashMap α β).get? a = none := by
+  simp [get?]
 
 @[simp]
-theorem find?_emptyc {a : α} : (∅ : HashMap α β).find? a = none := by
-  simp [find?]
+theorem get?_emptyc {a : α} : (∅ : HashMap α β).get? a = none := by
+  simp [get?]
 
-theorem findEntry?_insert {a k : α} {b : β} :
-    (m.insert a b).findEntry? k = bif a == k then some (a, b) else m.findEntry? k := by
-  simp [findEntry?, insert, DHashMap.findEntry?_insert, apply_bif (Option.map Sigma.toProd)]
+theorem getEntry?_insert {a k : α} {b : β} :
+    (m.insert a b).getEntry? k = bif a == k then some (a, b) else m.getEntry? k := by
+  simp [getEntry?, insert, DHashMap.getEntry?_insert, apply_bif (Option.map Sigma.toProd)]
 
-theorem find?_insert {a k : α} {b : β} :
-    (m.insert a b).find? k = bif a == k then some b else m.find? k := by
-  simp [find?, insert, DHashMap.findConst?_insert]
+theorem get?_insert {a k : α} {b : β} :
+    (m.insert a b).get? k = bif a == k then some b else m.get? k := by
+  simp [get?, insert, DHashMap.Const.get?_insert]
 
-theorem find?_congr {a b : α} (hab : a == b) : m.find? a = m.find? b := by
-  simp [find?, DHashMap.findConst?_congr _ hab]
+theorem get?_congr {a b : α} (hab : a == b) : m.get? a = m.get? b := by
+  simp [get?, DHashMap.Const.get?_congr _ hab]
 
 @[simp]
 theorem contains_empty {a : α} {c : Nat} : (empty c : HashMap α β).contains a = false := by
@@ -122,9 +122,9 @@ theorem contains_emptyc {a : α} : (∅ : HashMap α β).contains a = false := b
 theorem contains_insert {a k : α} {b : β} : (m.insert a b).contains k = ((a == k) || m.contains k) := by
   simp [contains, insert, DHashMap.contains_insert]
 
-theorem mem_values_iff_exists_find?_eq_some {β : Type v} (m : HashMap α β) {v : β} :
-    v ∈ m.values ↔ ∃ k, m.find? k = some v := by
-  simp [values, find?, DHashMap.mem_values_iff_exists_findConst?_eq_some]
+theorem mem_values_iff_exists_get?_eq_some {β : Type v} (m : HashMap α β) {v : β} :
+    v ∈ m.values ↔ ∃ k, m.get? k = some v := by
+  simp [values, get?, DHashMap.Const.mem_values_iff_exists_get?_eq_some]
 
 @[simp]
 theorem values_empty {β : Type v} {c} : (empty c : HashMap α β).values = [] := by
@@ -135,8 +135,8 @@ theorem values_emptyc {β : Type v} : (∅ : HashMap α β).values = [] := by
   simp [values]
 
 theorem mem_values_insert {β : Type v} {m : HashMap α β} {a : α} {b v : β} :
-    v ∈ (m.insert a b).values ↔ b = v ∨ ∃ k, (a == k) = false ∧ m.find? k = some v := by
-  simp [values, find?, insert, DHashMap.mem_values_insert]
+    v ∈ (m.insert a b).values ↔ b = v ∨ ∃ k, (a == k) = false ∧ m.get? k = some v := by
+  simp [values, get?, insert, DHashMap.mem_values_insert]
 
 end
 
